Finish _change_pf theorem and move full def to new file

proofs/core/RecFun.v
@@ -5,6 +5,14 @@ Require Export Denotational.
 
 Set Bullet Behavior "Strict Subproofs".
 
+(*Some results depend on proof irrelevance, which
+  follows anyway from LEM*)
+Lemma proof_irrel: forall (P: Prop) (H1 H2: P), H1 = H2.
+Proof.
+  apply ClassicalFacts.proof_irrelevance_cci;
+  apply Classical_Prop.classic.
+Qed.
+
 Section FunDef.
 
 
@@ -6189,6 +6197,256 @@ Variable vt: val_typevar.
   and [funcs_rep_aux] is not affected, as long as the two
   pf's agree on all fun/predsyms not in fs or ps*)
 
+Lemma get_arg_list_aux_change_pf: 
+  forall pf1 pf2 input ts rec1 rec2 v s small Hsmall hd Hhd vs Hparamslen
+      Hargslen Hall Hdec,
+    Forall (fun tm => forall ty small hd Hty Hdec Hsmall Hhd,
+      proj1_sig (@term_rep_aux vt pf1 input rec1 v tm ty small hd Hty Hdec Hsmall Hhd) =
+      proj1_sig (@term_rep_aux vt pf2 input rec2 v tm ty small hd Hty Hdec Hsmall Hhd))
+      ts ->
+    proj1_sig (@get_arg_list_ext_aux' vt v hd _ s
+      _ ts small Hsmall Hhd (term_rep_aux vt pf1 input rec1 v ) Hparamslen (s_args s) Hargslen Hall Hdec) =
+    proj1_sig (@get_arg_list_ext_aux' vt v hd _ s
+    vs ts small Hsmall Hhd (term_rep_aux vt pf2 input rec2 v ) Hparamslen (s_args s) Hargslen Hall Hdec).
+Proof.
+  intros pf1 pf2 input ts rec1 rec2 v s.
+  generalize dependent (s_args s). intros args; revert args.
+  induction ts; intros; simpl. 
+  - destruct args; simpl; auto.
+  - destruct args; simpl; [discriminate |].
+    inversion H; subst.
+    rewrite H2.
+    rewrite IHts. reflexivity.
+    auto.
+Qed.
+
+
+Lemma match_rep_addvars_change_pf input pf1 pf2 rec1 rec2 (t: term) ty1 pats:
+forall
+  v small hd (Hty1: term_has_type sigma t ty1) Hdec Hsmall Hhd (ty: vty) z Hall Hpats Halldec,
+  
+  term_rep_aux vt pf1 input rec1 v t ty1 small hd Hty1 Hdec Hsmall Hhd =
+  term_rep_aux vt pf2 input rec2 v t ty1 small hd Hty1 Hdec Hsmall Hhd ->
+
+  Forall (fun tm : term =>
+    forall (v: val_vars pd vt) (ty: vty)
+      (small: list vsymbol) (hd: option vsymbol) (Hty: term_has_type sigma tm ty)
+      (Hdec : decrease_fun fs ps small hd m vs tm) Hsmall Hhd,
+    term_rep_aux vt pf1 input rec1 v tm ty small hd Hty Hdec Hsmall Hhd =
+    term_rep_aux vt pf2 input rec2 v tm ty small hd Hty Hdec Hsmall Hhd)
+  (map snd pats) ->
+  @match_rep_addvars vt pf1 input rec1 v t _ small hd Hty1 Hdec Hsmall Hhd ty
+    z pats Hall Hpats Halldec =
+  @match_rep_addvars vt pf2 input rec2 v t _ small hd Hty1 Hdec Hsmall Hhd ty
+    z pats Hall Hpats Halldec.
+Proof.
+  induction pats; intros; simpl; auto.
+  destruct a; inversion H0; subst; rewrite IHpats; auto.
+  generalize dependent (@eq_refl _ (match_val_single gamma_valid pd all_unif vt ty1 p (Forall_inv Hpats)
+  (proj1_sig (term_rep_aux vt pf1 input rec1 v t ty1 small hd Hty1 Hdec Hsmall Hhd)))).
+  generalize dependent (@eq_refl _ (match_val_single gamma_valid pd all_unif vt ty1 p (Forall_inv Hpats)
+  (proj1_sig (term_rep_aux vt pf2 input rec2 v t ty1 small hd Hty1 Hdec Hsmall Hhd)))).
+  generalize dependent (@small_match_lemma vt t v ty1 p (Forall_inv Hpats)
+  (proj1_sig (term_rep_aux vt pf1 input rec1 v t ty1 small hd Hty1 Hdec Hsmall Hhd))
+  small (hide_ty
+  (dom_cast (dom_aux pd)
+     (arg_nth_eq vt (projT1 (projT2 (projT1 (projT1 input))))
+        (sn_sym (proj1_sig (projT1 (projT1 (projT1 input)))))
+        (sn_idx (proj1_sig (projT1 (projT1 (projT1 input)))))
+        (sn_idx_bound (proj1_sig (projT1 (projT1 (projT1 input))))
+           (proj2_sig (projT1 (projT1 (projT1 input))))))
+     (hnth (sn_idx (proj1_sig (projT1 (projT1 (projT1 input)))))
+        (projT2 (projT2 (projT1 (projT1 input)))) s_int 
+        (dom_int pd))))).
+  generalize dependent (@small_match_lemma vt t v ty1 p (Forall_inv Hpats)
+  (proj1_sig (term_rep_aux vt pf2 input rec2 v t ty1 small hd Hty1 Hdec Hsmall Hhd))
+  small (hide_ty
+  (dom_cast (dom_aux pd)
+      (arg_nth_eq vt (projT1 (projT2 (projT1 (projT1 input))))
+        (sn_sym (proj1_sig (projT1 (projT1 (projT1 input)))))
+        (sn_idx (proj1_sig (projT1 (projT1 (projT1 input)))))
+        (sn_idx_bound (proj1_sig (projT1 (projT1 (projT1 input))))
+            (proj2_sig (projT1 (projT1 (projT1 input))))))
+      (hnth (sn_idx (proj1_sig (projT1 (projT1 (projT1 input)))))
+        (projT2 (projT2 (projT1 (projT1 input)))) s_int 
+        (dom_int pd))))).
+  rewrite <- H.
+  (*One more generalization*)
+  generalize dependent (@match_val_single_upd_option vt v ty1
+  (proj1_sig (term_rep_aux vt pf1 input rec1 v t ty1 small hd Hty1 Hdec Hsmall Hhd)) p
+    (Forall_inv Hpats)).
+  (*Finally, we can destruct*)
+  destruct ( match_val_single gamma_valid pd all_unif vt ty1 p (Forall_inv Hpats)
+  (proj1_sig (term_rep_aux vt pf1 input rec1 v t ty1 small hd Hty1 Hdec Hsmall Hhd)));
+  intros.
+  - rewrite H3.
+    (*Use proof irrelevance*)
+    f_equal. f_equal;
+    apply proof_irrel.
+  - reflexivity.
+Qed.
+
+Lemma match_rep_rec_change_pf input pf1 pf2 rec1 rec2 (t: term) ty1 pats:
+forall
+  v small hd (Hty1: term_has_type sigma t ty1) Hdec Hsmall Hhd (ty: vty) Hall Hpats Halldec,
+  
+  term_rep_aux vt pf1 input rec1 v t ty1 small hd Hty1 Hdec Hsmall Hhd =
+  term_rep_aux vt pf2 input rec2 v t ty1 small hd Hty1 Hdec Hsmall Hhd ->
+
+  Forall (fun tm : term =>
+    forall (v: val_vars pd vt) (ty: vty)
+      (small: list vsymbol) (hd: option vsymbol) (Hty: term_has_type sigma tm ty)
+      (Hdec : decrease_fun fs ps small hd m vs tm) Hsmall Hhd,
+    term_rep_aux vt pf1 input rec1 v tm ty small hd Hty Hdec Hsmall Hhd =
+    term_rep_aux vt pf2 input rec2 v tm ty small hd Hty Hdec Hsmall Hhd)
+  (map snd pats) ->
+  @match_rep_rec vt pf1 input rec1 v t _ small hd Hty1 Hdec Hsmall Hhd ty
+    pats Hall Hpats Halldec =
+  @match_rep_rec vt pf2 input rec2 v t _ small hd Hty1 Hdec Hsmall Hhd ty
+    pats Hall Hpats Halldec.
+Proof.
+  induction pats; intros; simpl; auto.
+  destruct a; inversion H0; subst; rewrite IHpats; auto.
+  generalize dependent (@eq_refl _ (match_val_single gamma_valid pd all_unif vt ty1 p (Forall_inv Hpats)
+  (proj1_sig (term_rep_aux vt pf1 input rec1 v t ty1 small hd Hty1 Hdec Hsmall Hhd)))).
+  generalize dependent (@eq_refl _ (match_val_single gamma_valid pd all_unif vt ty1 p (Forall_inv Hpats)
+  (proj1_sig (term_rep_aux vt pf2 input rec2 v t ty1 small hd Hty1 Hdec Hsmall Hhd)))).
+  generalize dependent (@match_val_single_small1 vt v ty1 
+  (proj1_sig (term_rep_aux vt pf1 input rec1 v t ty1 small hd Hty1 Hdec Hsmall Hhd))
+  p (Forall_inv Hpats)). 
+  generalize dependent (@match_val_single_small1 vt v ty1 
+  (proj1_sig (term_rep_aux vt pf2 input rec2 v t ty1 small hd Hty1 Hdec Hsmall Hhd))
+  p (Forall_inv Hpats)). 
+  rewrite <- H.
+  (*One more generalization*)
+  generalize dependent (@match_val_single_upd_option vt v ty1
+  (proj1_sig (term_rep_aux vt pf1 input rec1 v t ty1 small hd Hty1 Hdec Hsmall Hhd)) p
+    (Forall_inv Hpats)).
+  (*Finally, we can destruct*)
+  destruct ( match_val_single gamma_valid pd all_unif vt ty1 p (Forall_inv Hpats)
+  (proj1_sig (term_rep_aux vt pf1 input rec1 v t ty1 small hd Hty1 Hdec Hsmall Hhd)));
+  intros.
+  - rewrite H3.
+    (*Use proof irrelevance*)
+    f_equal. f_equal;
+    apply proof_irrel.
+  - reflexivity.
+Qed.
+
+Lemma match_rep_addvars_change_pf' input pf1 pf2 rec1 rec2 (t: term) ty1 
+  (pats: list (pattern * formula)):
+forall
+  v small hd (Hty1: term_has_type sigma t ty1) Hdec Hsmall Hhd z Hall Hpats Halldec,
+  
+  term_rep_aux vt pf1 input rec1 v t ty1 small hd Hty1 Hdec Hsmall Hhd =
+  term_rep_aux vt pf2 input rec2 v t ty1 small hd Hty1 Hdec Hsmall Hhd ->
+
+  Forall (fun f : formula =>
+    forall (v: val_vars pd vt) 
+      (small: list vsymbol) (hd: option vsymbol) (Hval: valid_formula sigma f)
+      (Hdec : decrease_pred fs ps small hd m vs f) Hsmall Hhd,
+    formula_rep_aux vt pf1 input rec1 v f small hd Hval Hdec Hsmall Hhd =
+    formula_rep_aux vt pf2 input rec2 v f small hd Hval Hdec Hsmall Hhd)
+  (map snd pats) ->
+  @match_rep_addvars' vt pf1 input rec1 v t _ small hd Hty1 Hdec Hsmall Hhd
+    z pats Hall Hpats Halldec =
+  @match_rep_addvars' vt pf2 input rec2 v t _ small hd Hty1 Hdec Hsmall Hhd
+    z pats Hall Hpats Halldec.
+Proof.
+  induction pats; intros; simpl; auto.
+  destruct a; inversion H0; subst; rewrite IHpats; auto.
+  generalize dependent (@eq_refl _ (match_val_single gamma_valid pd all_unif vt ty1 p (Forall_inv Hpats)
+  (proj1_sig (term_rep_aux vt pf1 input rec1 v t ty1 small hd Hty1 Hdec Hsmall Hhd)))).
+  generalize dependent (@eq_refl _ (match_val_single gamma_valid pd all_unif vt ty1 p (Forall_inv Hpats)
+  (proj1_sig (term_rep_aux vt pf2 input rec2 v t ty1 small hd Hty1 Hdec Hsmall Hhd)))).
+  generalize dependent (@small_match_lemma vt t v ty1 p (Forall_inv Hpats)
+  (proj1_sig (term_rep_aux vt pf1 input rec1 v t ty1 small hd Hty1 Hdec Hsmall Hhd))
+  small (hide_ty
+  (dom_cast (dom_aux pd)
+     (arg_nth_eq vt (projT1 (projT2 (projT1 (projT1 input))))
+        (sn_sym (proj1_sig (projT1 (projT1 (projT1 input)))))
+        (sn_idx (proj1_sig (projT1 (projT1 (projT1 input)))))
+        (sn_idx_bound (proj1_sig (projT1 (projT1 (projT1 input))))
+           (proj2_sig (projT1 (projT1 (projT1 input))))))
+     (hnth (sn_idx (proj1_sig (projT1 (projT1 (projT1 input)))))
+        (projT2 (projT2 (projT1 (projT1 input)))) s_int 
+        (dom_int pd))))).
+  generalize dependent (@small_match_lemma vt t v ty1 p (Forall_inv Hpats)
+  (proj1_sig (term_rep_aux vt pf2 input rec2 v t ty1 small hd Hty1 Hdec Hsmall Hhd))
+  small (hide_ty
+  (dom_cast (dom_aux pd)
+      (arg_nth_eq vt (projT1 (projT2 (projT1 (projT1 input))))
+        (sn_sym (proj1_sig (projT1 (projT1 (projT1 input)))))
+        (sn_idx (proj1_sig (projT1 (projT1 (projT1 input)))))
+        (sn_idx_bound (proj1_sig (projT1 (projT1 (projT1 input))))
+            (proj2_sig (projT1 (projT1 (projT1 input))))))
+      (hnth (sn_idx (proj1_sig (projT1 (projT1 (projT1 input)))))
+        (projT2 (projT2 (projT1 (projT1 input)))) s_int 
+        (dom_int pd))))).
+  rewrite <- H.
+  (*One more generalization*)
+  generalize dependent (@match_val_single_upd_option vt v ty1
+  (proj1_sig (term_rep_aux vt pf1 input rec1 v t ty1 small hd Hty1 Hdec Hsmall Hhd)) p
+    (Forall_inv Hpats)).
+  (*Finally, we can destruct*)
+  destruct ( match_val_single gamma_valid pd all_unif vt ty1 p (Forall_inv Hpats)
+  (proj1_sig (term_rep_aux vt pf1 input rec1 v t ty1 small hd Hty1 Hdec Hsmall Hhd)));
+  intros.
+  - rewrite H3.
+    (*Use proof irrelevance*)
+    f_equal;
+    apply proof_irrel.
+  - reflexivity.
+Qed.
+
+Lemma match_rep_rec_change_pf' input pf1 pf2 rec1 rec2 (t: term) ty1 
+(pats: list (pattern * formula)):
+forall
+  v small hd (Hty1: term_has_type sigma t ty1) Hdec Hsmall Hhd Hall Hpats Halldec,
+  
+  term_rep_aux vt pf1 input rec1 v t ty1 small hd Hty1 Hdec Hsmall Hhd =
+  term_rep_aux vt pf2 input rec2 v t ty1 small hd Hty1 Hdec Hsmall Hhd ->
+
+  Forall (fun f : formula =>
+    forall (v: val_vars pd vt)
+      (small: list vsymbol) (hd: option vsymbol) (Hval: valid_formula sigma f)
+      (Hdec : decrease_pred fs ps small hd m vs f) Hsmall Hhd,
+    formula_rep_aux vt pf1 input rec1 v f small hd Hval Hdec Hsmall Hhd =
+    formula_rep_aux vt pf2 input rec2 v f small hd Hval Hdec Hsmall Hhd)
+  (map snd pats) ->
+  @match_rep_rec' vt pf1 input rec1 v t _ small hd Hty1 Hdec Hsmall Hhd
+    pats Hall Hpats Halldec =
+  @match_rep_rec' vt pf2 input rec2 v t _ small hd Hty1 Hdec Hsmall Hhd
+    pats Hall Hpats Halldec.
+Proof.
+  induction pats; intros; simpl; auto.
+  destruct a; inversion H0; subst; rewrite IHpats; auto.
+  generalize dependent (@eq_refl _ (match_val_single gamma_valid pd all_unif vt ty1 p (Forall_inv Hpats)
+  (proj1_sig (term_rep_aux vt pf1 input rec1 v t ty1 small hd Hty1 Hdec Hsmall Hhd)))).
+  generalize dependent (@eq_refl _ (match_val_single gamma_valid pd all_unif vt ty1 p (Forall_inv Hpats)
+  (proj1_sig (term_rep_aux vt pf2 input rec2 v t ty1 small hd Hty1 Hdec Hsmall Hhd)))).
+  generalize dependent (@match_val_single_small1 vt v ty1 
+  (proj1_sig (term_rep_aux vt pf1 input rec1 v t ty1 small hd Hty1 Hdec Hsmall Hhd))
+  p (Forall_inv Hpats)). 
+  generalize dependent (@match_val_single_small1 vt v ty1 
+  (proj1_sig (term_rep_aux vt pf2 input rec2 v t ty1 small hd Hty1 Hdec Hsmall Hhd))
+  p (Forall_inv Hpats)). 
+  rewrite <- H.
+  (*One more generalization*)
+  generalize dependent (@match_val_single_upd_option vt v ty1
+  (proj1_sig (term_rep_aux vt pf1 input rec1 v t ty1 small hd Hty1 Hdec Hsmall Hhd)) p
+    (Forall_inv Hpats)).
+  (*Finally, we can destruct*)
+  destruct ( match_val_single gamma_valid pd all_unif vt ty1 p (Forall_inv Hpats)
+  (proj1_sig (term_rep_aux vt pf1 input rec1 v t ty1 small hd Hty1 Hdec Hsmall Hhd)));
+  intros.
+  - rewrite H3.
+    (*Use proof irrelevance*)
+    f_equal;
+    apply proof_irrel.
+  - reflexivity.
+Qed.
+
 Theorem term_fmla_rep_change_pf (pf1 pf2: pi_funpred gamma_valid pd)
 (Hpf1: forall f srts a, ~ In f (map fn_sym fs) ->
   funs gamma_valid pd pf1 f srts a = funs gamma_valid pd pf2 f srts a)
@@ -6197,13 +6455,13 @@ Theorem term_fmla_rep_change_pf (pf1 pf2: pi_funpred gamma_valid pd)
 (t: term) (f: formula) :
 (forall 
   (input: packed_args2 vt)
-  (rec: (forall 
+  (*(rec: (forall 
   (y : packed_args2 vt),
   R_projT1 _(R_projT1 _  (arg_list_smaller vt)) y input  -> 
-  funrep_ret (projT1 y)))
+  funrep_ret (projT1 y)))*)
   (IH:forall (y: packed_args2 vt)
   (small: R_projT1 _ (R_projT1 _ (arg_list_smaller vt)) y input),
-  rec y small = funcs_rep_aux vt pf2 y)
+  funcs_rep_aux vt pf1 y = funcs_rep_aux vt pf2 y)
   (v: val_vars pd vt) (*TODO: I think we don't need a condition
     here bc we prove equality*)
   (*TODO: what conditions on the term?*)
@@ -6239,16 +6497,16 @@ Theorem term_fmla_rep_change_pf (pf1 pf2: pi_funpred gamma_valid pd)
               (projT2 (projT2 (projT1 (projT1 input)))) s_int 
               (dom_int pd)))),
 
-  term_rep_aux vt pf1 input rec v t ty small hd Hty Hdec Hsmall Hhd =
-  term_rep_aux vt pf2 input rec v t ty small hd Hty Hdec Hsmall Hhd
+  term_rep_aux vt pf1 input (fun x _ => funcs_rep_aux vt pf1 x) v t ty small hd Hty Hdec Hsmall Hhd =
+  term_rep_aux vt pf2 input (fun x _ => funcs_rep_aux vt pf2 x) v t ty small hd Hty Hdec Hsmall Hhd
 ) /\
 (forall (input: packed_args2 vt)
-  (rec: (forall (y : packed_args2 vt),
+  (*(rec: (forall (y : packed_args2 vt),
   R_projT1 _(R_projT1 _  (arg_list_smaller vt)) y input -> 
-  funrep_ret (projT1 y)))
+  funrep_ret (projT1 y)))*)
   (IH:forall (y: packed_args2 vt)
   (small: R_projT1 _ (R_projT1 _ (arg_list_smaller vt)) y input),
-  rec y small = funcs_rep_aux vt pf2 y)
+  funcs_rep_aux vt pf1 y = funcs_rep_aux vt pf2 y)
   (v: val_vars pd vt) (*TODO: I think we don't need a condition
     here bc we prove equality*)
   (*TODO: what conditions on the term?*)
@@ -6284,14 +6542,125 @@ Theorem term_fmla_rep_change_pf (pf1 pf2: pi_funpred gamma_valid pd)
               (projT2 (projT2 (projT1 (projT1 input)))) s_int 
               (dom_int pd)))),
 
-  formula_rep_aux vt pf1 input rec v f small hd Hval Hdec Hsmall Hhd =
-  formula_rep_aux vt pf2 input rec v f small hd Hval Hdec Hsmall Hhd
+  formula_rep_aux vt pf1 input (fun x _ => funcs_rep_aux vt pf1 x) v f small hd Hval Hdec Hsmall Hhd =
+  formula_rep_aux vt pf2 input (fun x _ => funcs_rep_aux vt pf2 x) v f small hd Hval Hdec Hsmall Hhd
 )
 .
 Proof.
-  (*TODO: is this theorem correct? What should rec be?*)
-Admitted.
-
+  revert t f.
+  apply term_formula_ind; intros (*don't solve trivial,
+    takes too long to "try"*).
+  - reflexivity.
+  - reflexivity.
+  - (*Tfun case*)
+    rewrite !term_rep_aux_fun. cbn zeta.
+    destruct (find_fn f1 fs).
+    + rewrite IH.
+      match goal with
+      | |- exist ?a ?b ?c = exist ?a ?b1 ?c1 =>
+        let H := fresh in
+        assert (H: b = b1); [|rewrite H; reflexivity]
+      end.
+      (*unfold cast_dom_vty.
+      rewrite !dom_cast_compose.*)
+      rewrite get_arg_list_aux_change_pf with(pf2:=pf2)
+      (rec2:=(fun x _ => funcs_rep_aux vt pf2 x)).
+      reflexivity. 
+      revert H; rewrite !Forall_forall; intros.
+      rewrite H; auto.
+      (*Prove that this is smaller*)
+      apply func_smaller_case'.
+    + match goal with
+      | |- exist ?a ?b ?c = exist ?a ?b1 ?c1 =>
+        let H := fresh in
+        assert (H: b = b1); [|rewrite H; reflexivity]
+      end.
+      rewrite get_arg_list_aux_change_pf with(pf2:=pf2)
+      (rec2:=(fun x _ => funcs_rep_aux vt pf2 x)).
+      rewrite Hpf1.
+      reflexivity. auto. 
+      revert H; rewrite !Forall_forall; intros.
+      rewrite H; auto.
+  - simpl. rewrite H, H0; auto.
+  - simpl. rewrite H; auto.
+    match goal with 
+    | |- context [if ?b then ?c1 else ?c2] => destruct b
+    end.
+    + match goal with
+      | |- exist _ ?x ?H1 = exist _ ?y ?H2 =>
+        let H := fresh in
+        assert (H: x = y); [|rewrite H; reflexivity]
+      end.
+      rewrite H0; auto.
+    + match goal with
+      | |- exist _ ?x ?H1 = exist _ ?y ?H2 =>
+        let H := fresh in
+        assert (H: x = y); [|rewrite H; reflexivity]
+      end.
+      rewrite H1; auto.
+  - (*Tmatch case*)
+    rewrite !term_rep_aux_match. cbn zeta.
+    destruct (tmatch_case tm hd small).
+    +  match goal with
+      | |- exist _ ?x ?H1 = exist _ ?y ?H2 =>
+        let H := fresh in
+        assert (H: x = y); [|rewrite H; reflexivity]
+      end.
+      apply match_rep_addvars_change_pf.
+      auto. 
+      revert H0; rewrite !Forall_forall; intros; apply H0; auto.
+    +  match goal with
+      | |- exist _ ?x ?H1 = exist _ ?y ?H2 =>
+        let H := fresh in
+        assert (H: x = y); [|rewrite H; reflexivity]
+      end.
+      apply match_rep_rec_change_pf; auto.
+      revert H0; rewrite !Forall_forall; intros; apply H0; auto.
+  - simpl.
+    match goal with
+    | |- exist _ ?x ?H1 = exist _ ?y ?H2 =>
+      let H := fresh in
+      assert (H: x = y); [|rewrite H; reflexivity]
+    end.
+    f_equal.
+    apply functional_extensionality_dep; intros.
+    rewrite H. reflexivity. auto.
+  - (*Fpred*)
+    rewrite !formula_rep_aux_pred.  
+    cbn zeta.
+    destruct (find_pn p ps).
+    + rewrite IH by apply pred_smaller_case'.
+      rewrite get_arg_list_aux_change_pf with(pf2:=pf2)
+      (rec2:=(fun x _ => funcs_rep_aux vt pf2 x)).
+      reflexivity. 
+      revert H; rewrite !Forall_forall; intros;
+      rewrite H; auto.
+    + rewrite get_arg_list_aux_change_pf with(pf2:=pf2)
+      (rec2:=(fun x _ => funcs_rep_aux vt pf2 x)).
+      rewrite Hpf2; auto.
+      revert H; rewrite !Forall_forall; intros;
+      rewrite H; auto.
+  - simpl; destruct q; apply all_dec_eq; split;
+    [intros Hd d; specialize (Hd d) | intros Hd d;
+      specialize (Hd d) | intros [d Hd]; exists d | intros [d Hd]; exists d];
+    try solve[rewrite H; auto]; 
+    try solve[rewrite <- H; auto].
+  - simpl; rewrite H, H0; auto.
+  - simpl; rewrite H, H0; auto.
+  - simpl; rewrite H; auto.
+  - reflexivity.
+  - reflexivity.
+  - simpl; rewrite H, H0; auto.
+  - simpl; rewrite H, H0, H1; auto.
+  - (*Fmatch*)
+    rewrite !formula_rep_aux_match. cbn zeta.
+    destruct (tmatch_case tm hd small).
+    + apply match_rep_addvars_change_pf'.
+      auto. 
+      revert H0; rewrite !Forall_forall; intros; apply H0; auto.
+    + apply match_rep_rec_change_pf'; auto.
+      revert H0; rewrite !Forall_forall; intros; apply H0; auto.
+Qed.
 
 Theorem funcs_rep_aux_change_pf 
   (pf1 pf2: pi_funpred gamma_valid pd)
@@ -6317,1058 +6686,10 @@ Proof.
       a goal only about the [term_rep] and [term_rep_aux]*)
     f_equal.
     rewrite (proj1 (term_fmla_rep_change_pf pf1 pf2 Hpf1 Hpf2 _ Ftrue)).
-    f_equal.
-    (*f_equal takes a long time (> 20 seconds), so we do the following*)
-    match goal with
-    | |- term_rep_aux ?vt ?pf ?input ?f1 ?val ?t ?ty ?small ?hd ?Hty ?Hdec
-      ?Hsmall ?Hhd =
-      term_rep_aux ?vt ?pf ?input ?f2 ?val ?t ?ty ?small ?hd ?Hty ?Hdec
-      ?Hsmall ?Hhd =>
-      let H := fresh in
-      assert (H: f1 = f2) by (repeat (apply functional_extensionality_dep; intros);
-        apply IH; auto); rewrite H; reflexivity
-    end.
-    apply IH.
+    reflexivity. auto.
   - rewrite !funcs_rep_aux_eq. simpl.
     rewrite (proj2 (term_fmla_rep_change_pf pf1 pf2 Hpf1 Hpf2 tm_d _)).
-    (*We do the same to avoid f_equal*)    
-    match goal with
-    | |- formula_rep_aux ?vt ?pf ?input ?f1 ?val ?t ?small ?hd ?Hty ?Hdec
-      ?Hsmall ?Hhd =
-      formula_rep_aux ?vt ?pf ?input ?f2 ?val ?t ?small ?hd ?Hty ?Hdec
-      ?Hsmall ?Hhd =>
-      let H := fresh in
-      assert (H: f1 = f2) by (repeat (apply functional_extensionality_dep; intros);
-        apply IH; auto); rewrite H; reflexivity
-    end.
-    apply IH.
+    reflexivity. auto.
 Qed.
 
 End FunDef.
-
-(*Now we give the full definition*)
-Section Full.
-
-(*First, we define when a mutual function body is in a context*)
-
-(*TODO: move*)
-
-(*Similar to mutual types*)
-
-Definition funsym_in_mutfun (f: funsym) (l: list funpred_def) : bool :=
-  in_bool funsym_eq_dec f (funsyms_of_def (recursive_def l)).
-
-Definition get_mutfun_fun (f: funsym) (gamma': context) : option (list funpred_def) :=
-  find (funsym_in_mutfun f) (mutfuns_of_context gamma').
-
-Definition predsym_in_mutfun (p: predsym) (l: list funpred_def) : bool :=
-  in_bool predsym_eq_dec p (predsyms_of_def (recursive_def l)).
-
-Definition get_mutfun_pred (p: predsym) (gamma': context) : option (list funpred_def) :=
-  find (predsym_in_mutfun p) (mutfuns_of_context gamma').
-
-
-
-Context {sigma: sig} {gamma: context} (gamma_valid: valid_context sigma gamma)
-{pd: pi_dom} (all_unif: forall m, mut_in_ctx m gamma -> IndTypes.uniform m).
-
-
-
-(*TODO: move to typing*)
-
-Lemma funpred_def_valid (l: list funpred_def)
-  (l_in: In l (mutfuns_of_context gamma)):
-  funpred_valid_type sigma gamma l.
-Proof.
-  destruct gamma_valid.
-  rewrite Forall_forall in H0.
-  rewrite in_mutfuns_spec in l_in.
-  specialize (H0 _ l_in). exact H0.
-Qed.
-
-Lemma funpred_defs_to_sns_types l il:
-  length l = length il ->
-  In l (mutfuns_of_context gamma) ->
-  Forall (fun f => term_has_type sigma (fn_body f) (f_ret (fn_sym f))) 
-    (fst (funpred_defs_to_sns l il)).
-Proof.
-  intros. apply funpred_def_valid in H0.
-  unfold funpred_valid_type in H0.
-  destruct H0.
-  rewrite Forall_forall.
-  intros x. rewrite funpred_defs_to_sns_in_fst; auto.
-  intros [i [Hi Hx]].
-  rewrite Forall_forall in H0.
-  set (y:=nth i (fst (split_funpred_defs l)) (id_fs, [], tm_d)) in *.
-  simpl in Hx.
-  subst. 
-  assert (In (fun_def (fst (fst y)) (snd (fst y)) (snd y)) l). {
-    apply (split_funpred_defs_in_l l). subst y. apply nth_In. auto.
-  }
-  apply H0 in H2. simpl in H2.
-  destruct_all. unfold well_typed_term in H2.
-  destruct H2.
-  simpl. apply H2.
-Qed.
-
-Lemma funpred_defs_to_sns_valid l il:
-  length l = length il ->
-  In l (mutfuns_of_context gamma) ->
-  Forall (fun p => valid_formula sigma (pn_body p)) 
-    (snd (funpred_defs_to_sns l il)).
-Proof.
-  intros. apply funpred_def_valid in H0.
-  unfold funpred_valid_type in H0.
-  destruct H0.
-  rewrite Forall_forall.
-  intros x. rewrite funpred_defs_to_sns_in_snd; auto.
-  intros [i [Hi Hx]].
-  rewrite Forall_forall in H0.
-  set (y:=nth i (snd (split_funpred_defs l)) (id_ps, [], Ftrue)) in *.
-  simpl in Hx.
-  subst. simpl. 
-  assert (In (pred_def (fst (fst y)) (snd (fst y)) (snd y)) l). {
-    apply (split_funpred_defs_in_l l). subst y. apply nth_In. auto.
-  }
-  apply H0 in H2. simpl in H2.
-  destruct_all. unfold well_typed_term in H2.
-  destruct H2. auto.
-Qed.
-
-(*Prove the typevar condition
-  This proof is annoying because there is so much unfolding
-  and proving equivalences between being "in" different lists,
-  but it it not too hard*)
-Lemma funpred_defs_to_sns_typevars1 {l: list funpred_def} 
-  {il: list nat} {params: list typevar}
-  (l_in: In l (mutfuns_of_context gamma))
-  (Hparams: forall f : fn,
-    In f (fst (funpred_defs_to_sns l il)) ->
-    s_params (fn_sym f) = params):
-  length l = length il ->
-  (forall f : fn,
-  In f (fst (funpred_defs_to_sns l il)) ->
-  forall ty : vty,
-  In ty (f_ret (fn_sym f) :: s_args (fn_sym f)) ->
-  forall x : typevar, In x (type_vars ty) -> In x params).
-Proof.
-  intros Hlen. intros.
-  destruct gamma_valid as [Hwf _].
-  unfold wf_context in Hwf.
-  destruct Hwf as [Hwf [_ [Hallin _]]].
-  unfold wf_sig in Hwf. destruct Hwf as [Halltyp _].
-  rewrite Forall_forall in Hallin.
-  assert (Hin:=H).
-  rewrite funpred_defs_to_sns_in_fst in H; auto.
-  destruct H as [i [Hi Hf]].
-  set (y:=nth i (fst (split_funpred_defs l)) (id_fs, [], tm_d)) in *.
-  simpl in Hf.
-  subst. simpl in H0.
-  assert (In (fun_def (fst (fst y)) (snd (fst y)) (snd y)) l). {
-    apply (split_funpred_defs_in_l l). subst y. apply nth_In. auto.
-  }
-  assert (Hinf: In (fst (fst y)) (funsyms_of_context gamma)). {
-    unfold funsyms_of_context. rewrite in_concat.
-    exists (funsyms_of_def (recursive_def l)). split; auto.
-    rewrite in_map_iff. exists (recursive_def l); split; auto.
-    apply in_mutfuns_spec; auto.
-    clear -H. generalize dependent y; intros.
-    simpl. induction l; simpl; [inversion H |]. destruct a; simpl; auto;
-    destruct H; simpl; auto; inversion H; subst; auto.
-  }
-  specialize (Hallin _ Hinf).
-  rewrite Forall_forall in Halltyp.
-  specialize (Halltyp _ Hallin).
-  rewrite Forall_forall in Halltyp.
-  specialize (Halltyp ty H0). destruct Halltyp as [Hvalty Hallty].
-  rewrite Forall_forall in Hallty.
-  rewrite <- (Hparams _ Hin). simpl. apply Hallty. auto.
-Qed.
-
-Lemma funpred_defs_to_sns_typevars2 {l: list funpred_def} 
-  {il: list nat} {params: list typevar}
-  (l_in: In l (mutfuns_of_context gamma))
-  (Hparams: forall p : pn,
-    In p (snd (funpred_defs_to_sns l il)) ->
-    s_params (pn_sym p) = params):
-  length l = length il ->
-  (forall p : pn,
-  In p (snd (funpred_defs_to_sns l il)) ->
-  forall ty : vty,
-  In ty (s_args (pn_sym p)) ->
-  forall x : typevar, In x (type_vars ty) -> In x params).
-Proof.
-  intros Hlen. intros.
-  destruct gamma_valid as [Hwf _].
-  unfold wf_context in Hwf.
-  destruct Hwf as [Hwf [_ [_ [Hallin _]]]].
-  unfold wf_sig in Hwf. destruct Hwf as [_ Halltyp].
-  rewrite Forall_forall in Hallin.
-  assert (Hin:=H).
-  rewrite funpred_defs_to_sns_in_snd in H; auto.
-  destruct H as [i [Hi Hf]].
-  set (y:=nth i (snd (split_funpred_defs l)) (id_ps, [], Ftrue)) in *.
-  simpl in Hf.
-  rewrite map_length in Hf.
-  replace (length (combine (fst (split_funpred_defs l))
-  (firstn (Datatypes.length (fst (split_funpred_defs l))) il))) with
-  (length (fst (split_funpred_defs l))) in Hf by
-    (rewrite combine_length, firstn_length;
-    pose proof (split_funpred_defs_length l); lia).
-  subst. simpl in H0.
-  assert (In (pred_def (fst (fst y)) (snd (fst y)) (snd y)) l). {
-    apply (split_funpred_defs_in_l l). subst y. apply nth_In. auto.
-  }
-  assert (Hinf: In (fst (fst y)) (predsyms_of_context gamma)). {
-    unfold predsyms_of_context. rewrite in_concat.
-    exists (predsyms_of_def (recursive_def l)). split; auto.
-    rewrite in_map_iff. exists (recursive_def l); split; auto.
-    apply in_mutfuns_spec; auto.
-    clear -H. generalize dependent y; intros.
-    simpl. induction l; simpl; [inversion H |]. destruct a; simpl; auto;
-    destruct H; simpl; auto; inversion H; subst; auto.
-  }
-  specialize (Hallin _ Hinf).
-  rewrite Forall_forall in Halltyp.
-  specialize (Halltyp _ Hallin).
-  rewrite Forall_forall in Halltyp.
-  specialize (Halltyp ty H0). destruct Halltyp as [Hvalty Hallty].
-  rewrite Forall_forall in Hallty.
-  rewrite <- (Hparams _ Hin). simpl. apply Hallty. auto.
-Qed.
-
-Lemma get_funsym_fn {l: list funpred_def} {il} {f: funsym}
-  (l_in: In l (mutfuns_of_context gamma))
-  (f_in: funsym_in_mutfun f l):
-  length l = length il ->
-  { f' : fn | In f' (fst (funpred_defs_to_sns l il)) /\ 
-    f = fn_sym f' }.
-Proof.
-  intros.
-  destruct (find_fn f (fst (funpred_defs_to_sns l il))); auto.
-  (*Just need to show contradiction case - we can use Props here*)
-  exfalso.
-  apply n.
-  clear n.
-  apply in_bool_In in f_in.
-  assert ((fold_right
-  (fun (x : funpred_def) (acc : list funsym) =>
-   match x with
-   | fun_def f' _ _ => f' :: acc
-   | pred_def _ _ _ => acc
-   end) [] l) = (map fn_sym (fst (funpred_defs_to_sns l il)))). {
-    unfold funpred_defs_to_sns; simpl.
-    pose proof (split_funpred_defs_length l).
-    rewrite !map_map. simpl. rewrite map_fst_fst_fst_combine by
-      (rewrite firstn_length; lia).
-    clear. induction l; simpl; auto; destruct a; simpl; auto.
-    f_equal; auto.
-  }
-  rewrite <- H0; auto.
-Qed.
-
-Lemma get_predsym_pn {l: list funpred_def} {il} {p: predsym}
-  (l_in: In l (mutfuns_of_context gamma))
-  (p_in: predsym_in_mutfun p l):
-  length l = length il ->
-  { p' : pn | In p' (snd (funpred_defs_to_sns l il)) /\ 
-    p = pn_sym p' }.
-Proof.
-  intros.
-  destruct (find_pn p (snd (funpred_defs_to_sns l il))); auto.
-  (*Just need to show contradiction case - we can use Props here*)
-  exfalso.
-  apply n.
-  clear n.
-  apply in_bool_In in p_in.
-  assert ((fold_right
-  (fun (x : funpred_def) (acc : list predsym) =>
-   match x with
-   | fun_def _ _ _ => acc
-   | pred_def p' _ _ => p' :: acc
-   end) [] l) = (map pn_sym (snd (funpred_defs_to_sns l il)))). {
-    unfold funpred_defs_to_sns; simpl.
-    pose proof (split_funpred_defs_length l).
-    rewrite !map_map. simpl. rewrite map_fst_fst_fst_combine by
-      (rewrite skipn_length; lia).
-    clear. induction l; simpl; auto; destruct a; simpl; auto.
-    f_equal; auto.
-  }
-  rewrite <- H0; auto.
-Qed.
-
-(*Get fs and ps associated with a funpred_def*)
-Definition get_funpred_def_info (l: list funpred_def)
-  (l_in: In l (mutfuns_of_context gamma)):
-  (list fn * list pn).
-Proof.
-  pose proof (funpred_def_valid _ l_in) as Hval.
-  unfold funpred_valid_type in Hval.
-  destruct Hval.
-  (*Here, we use the typechecking result that it is
-    decidable to find the list of indices*)
-  apply (Typechecker.funpred_def_term_decide sigma gamma (proj1 gamma_valid) _ l_in) 
-  in H0.
-  destruct H0 as [t Ht].
-  exact (funpred_defs_to_sns l (snd t)).
-Defined.
-
-(*We will need to prove that this has all of the desired properties*)
-
-
-Notation domain := (domain (dom_aux pd)).
-
-(*Here, we fix our valuation since we cannot take in any
-  input in our final version. We can give a trivial valuation
-  and define the mapping on the typesyms and vsyms that we care
-  about. We will need to show it equals a [term_rep] and [formula_rep]
-  for an arbirtary valuation, which will require a bit of annoying casting*)
-
-
-(*Definition of funs_rep - what we will set each recursive function
-  to in our full interp.
-  The difficulty in defining this is in showing that all of the
-  conditions we need about fs and ps are satisfied; they
-  all follow, in one way or another, from the wf context and/or
-  the typechecker's correctness.
-  We need a pf to know how to evaluate other function and
-  predicate symbols (non-recursive ones)*)
-Definition funs_rep (pf: pi_funpred gamma_valid pd) 
-  (f: funsym) (l: list funpred_def)
-  (f_in: funsym_in_mutfun f l)
-  (l_in: In l (mutfuns_of_context gamma))
-  (srts: list sort)
-  (srts_len: length srts = length (s_params f))
-  (a: arg_list domain (sym_sigma_args f srts)):
-  domain (funsym_sigma_ret f srts).
-(*TODO: manual definition?*)
-Proof.
-  pose proof (funpred_def_valid _ l_in) as Hval.
-  destruct Hval as [Hval Hex].
-  apply (Typechecker.funpred_def_term_decide sigma gamma (proj1 gamma_valid) _ l_in) 
-  in Hex.
-  destruct Hex as [t Ht].
-  set (sns := (funpred_defs_to_sns l (snd t))).
-  unfold funpred_def_term in Ht.
-  destruct Ht as [Hnotnil [Hlenparams [m_in [Hlen [Hidx [Hfvty [Hpvty [Hfparams [Hpparams [Hfdec Hpdec]]]]]]]]]].
-  set (vt:=(vt_with_args triv_val_typevar (snd (fst (fst t))) srts)).
-  set (fn_info := get_funsym_fn l_in f_in (eq_sym Hlen)).
-  assert (Hsrtslen': Datatypes.length srts = Datatypes.length (snd (fst (fst t)))). {
-    rewrite srts_len, (proj2' (proj2_sig fn_info)), 
-    (Hfparams _ (proj1' (proj2_sig fn_info))).
-    reflexivity.
-  }
-  assert (Hparamsnodup: NoDup (snd (fst (fst t)))). {
-    rewrite <- (Hfparams _ (proj1' (proj2_sig fn_info))).
-    apply s_params_Nodup.
-  }
-  set (Heqf :=
-  eq_trans (f_equal f_sym (proj2' (proj2_sig fn_info)))
-  (fs_wf_eq _ (proj1' (funpred_def_to_sns_wf sigma gamma l (snd t) Hlen Hidx Hval))
-  _ (proj1' (proj2_sig fn_info))) : f_sym f = sn_sym (proj1_sig fn_info) ).
-  set (a':= (cast_arg_list (f_equal (fun x => sym_sigma_args x srts) Heqf) a)).
-  (*Need to get the fn associated with this funsym*)
-  (*We call [funs_rep_aux] with all of the proofs we need; we need
-    to cast the result because it returns something basedon the funsym*)
-  exact (dom_cast _ 
-    (f_equal (fun x => funsym_sigma_ret x srts) (eq_sym (proj2 (proj2_sig fn_info))))
-
-  (@funs_rep_aux _ _ gamma_valid pd all_unif (fst sns) (snd sns)
-    (proj1' (funpred_def_to_sns_wf sigma gamma l (snd t) Hlen Hidx Hval))
-    (proj2' (funpred_def_to_sns_wf sigma gamma l (snd t) Hlen Hidx Hval))
-    (proj1' (funpred_defs_to_sns_NoDup (proj1 gamma_valid) _ _ l_in (eq_sym Hlen)))
-    (proj2' (funpred_defs_to_sns_NoDup (proj1 gamma_valid) _ _ l_in (eq_sym Hlen)))
-    (funpred_defs_to_sns_types _ _ (eq_sym Hlen) l_in)
-    (funpred_defs_to_sns_valid _ _ (eq_sym Hlen) l_in)
-    (snd (fst (fst t))) Hfparams Hpparams
-    (funpred_defs_to_sns_typevars1 l_in Hfparams (eq_sym Hlen))
-    (funpred_defs_to_sns_typevars2 l_in Hpparams (eq_sym Hlen))
-    (fst (fst (fst t))) (snd (fst t)) Hlenparams Hfvty Hpvty Hfdec Hpdec 
-      m_in (*pf*) _ pf (triv_val_vars pd vt)
-    (proj1_sig fn_info)
-    (proj1' (proj2_sig fn_info))
-    srts Hsrtslen'
-    (vt_with_args_vt_eq _ _ Hparamsnodup Hsrtslen')
-    a')).
-Defined.
-
-(*preds_rep*)
-Definition preds_rep (pf: pi_funpred gamma_valid pd) 
-  (p: predsym) (l: list funpred_def)
-  (p_in: predsym_in_mutfun p l)
-  (l_in: In l (mutfuns_of_context gamma))
-  (srts: list sort)
-  (srts_len: length srts = length (s_params p))
-  (a: arg_list domain (sym_sigma_args p srts)):
-  bool.
-(*TODO: manual definition?*)
-Proof.
-  pose proof (funpred_def_valid _ l_in) as Hval.
-  destruct Hval as [Hval Hex].
-  apply (Typechecker.funpred_def_term_decide sigma gamma (proj1 gamma_valid) _ l_in) 
-  in Hex.
-  destruct Hex as [t Ht].
-  set (sns := (funpred_defs_to_sns l (snd t))).
-  unfold funpred_def_term in Ht.
-  destruct Ht as [Hnotnil [Hlenparams [m_in [Hlen [Hidx [Hfvty [Hpvty [Hfparams [Hpparams [Hfdec Hpdec]]]]]]]]]].
-  set (vt:=(vt_with_args triv_val_typevar (snd (fst (fst t))) srts)).
-  set (pn_info := get_predsym_pn l_in p_in (eq_sym Hlen)).
-  assert (Hsrtslen': Datatypes.length srts = Datatypes.length (snd (fst (fst t)))). {
-    rewrite srts_len, (proj2 (proj2_sig pn_info)), 
-    (Hpparams _ (proj1 (proj2_sig pn_info))).
-    reflexivity.
-  }
-  assert (Hparamsnodup: NoDup (snd (fst (fst t)))). {
-    rewrite <- (Hpparams _ (proj1 (proj2_sig pn_info))).
-    apply s_params_Nodup.
-  }
-  set (Heqf :=
-  eq_trans (f_equal p_sym (proj2 (proj2_sig pn_info)))
-  (ps_wf_eq _ (proj2 (funpred_def_to_sns_wf sigma gamma l (snd t) Hlen Hidx Hval))
-  _ (proj1 (proj2_sig pn_info))) : p_sym p = sn_sym (proj1_sig pn_info) ).
-  set (a':= (cast_arg_list (f_equal (fun x => sym_sigma_args x srts) Heqf) a)).
-  (*Need to get the fn associated with this funsym*)
-  (*We call [funs_rep_aux] with all of the proofs we need; we need
-    to cast the result because it returns something basedon the funsym*)
-  exact (@preds_rep_aux _ _ gamma_valid pd all_unif (fst sns) (snd sns)
-    (proj1 (funpred_def_to_sns_wf sigma gamma l (snd t) Hlen Hidx Hval))
-    (proj2 (funpred_def_to_sns_wf sigma gamma l (snd t) Hlen Hidx Hval))
-    (proj1 (funpred_defs_to_sns_NoDup (proj1 gamma_valid) _ _ l_in (eq_sym Hlen)))
-    (proj2 (funpred_defs_to_sns_NoDup (proj1 gamma_valid) _ _ l_in (eq_sym Hlen)))
-    (funpred_defs_to_sns_types _ _ (eq_sym Hlen) l_in)
-    (funpred_defs_to_sns_valid _ _ (eq_sym Hlen) l_in)
-    (snd (fst (fst t))) Hfparams Hpparams
-    (funpred_defs_to_sns_typevars1 l_in Hfparams (eq_sym Hlen))
-    (funpred_defs_to_sns_typevars2 l_in Hpparams (eq_sym Hlen))
-    (fst (fst (fst t))) (snd (fst t)) Hlenparams Hfvty Hpvty Hfdec Hpdec 
-      m_in _ pf (triv_val_vars pd vt)
-    (proj1_sig pn_info)
-    (proj1 (proj2_sig pn_info))
-    srts Hsrtslen'
-    (vt_with_args_vt_eq _ _ Hparamsnodup Hsrtslen')
-    a').
-Defined.
-
-Lemma funsym_in_mutfun_dec: forall f l, { funsym_in_mutfun f l} + {~ funsym_in_mutfun f l}.
-Proof.
-  intros. destruct (funsym_in_mutfun f l) eqn : Ha. auto. right.
-  intro C; inversion C.
-Qed.
-
-Lemma predsym_in_mutfun_dec: forall p l, { predsym_in_mutfun p l} + 
-  {~ predsym_in_mutfun p l}.
-Proof.
-  intros. destruct (predsym_in_mutfun p l) eqn : Ha. auto. right.
-  intro C; inversion C.
-Qed.
-
-(*Now we define a modified pi_funpred, where we interpret
-  these functions and predicates using their reps*)
-Definition funpred_with_reps_funs (pf: pi_funpred gamma_valid pd)
-  (l: list funpred_def)
-  (l_in: In l (mutfuns_of_context gamma)) :
-  forall (f: funsym) (srts: list sort)
-  (a: arg_list domain (sym_sigma_args f srts)),
-  domain (funsym_sigma_ret f srts) :=
-
-  (*Need to see if f in l and srts has right length*)
-  fun f srts a => 
-    match funsym_in_mutfun_dec f l with (*funsym_in_mutfun f l as b return funsym_in_mutfun f l = b -> 
-      domain (funsym_sigma_ret f srts) *)
-    | left f_in => 
-      (*TODO: should we require srts_len always?*)
-      match (Nat.eq_dec (length srts) (length (s_params f) )) with
-      | left srts_len =>
-        funs_rep pf f l f_in l_in srts srts_len a
-      | right srts_len => (funs gamma_valid pd pf) f srts a
-      end
-    | right f_notin => (funs gamma_valid pd pf) f srts a
-    end.
-
-Definition funpred_with_reps_preds (pf: pi_funpred gamma_valid pd)
-  (l: list funpred_def)
-  (l_in: In l (mutfuns_of_context gamma)) :
-  forall (p: predsym) (srts: list sort)
-  (a: arg_list domain (sym_sigma_args p srts)),
-  bool :=
-
-  (*Need to see if f in l and srts has right length*)
-  fun p srts a => 
-    match predsym_in_mutfun_dec p l with
-    | left p_in =>
-      (*TODO: should we require srts_len always?*)
-      match (Nat.eq_dec (length srts) (length (s_params p) ))with
-      | left srts_len =>
-        preds_rep pf p l p_in l_in srts srts_len a
-      | right srts_len => (preds gamma_valid pd pf) p srts a
-      end
-    | right p_notin => (preds gamma_valid pd pf) p srts a
-    end.
-
-Lemma constr_in_adt_def a m f:
-  adt_in_mut a m ->
-  constr_in_adt f a ->
-  In f (funsyms_of_def (datatype_def m)).
-Proof.
-  unfold mut_in_ctx. unfold adt_in_mut. unfold constr_in_adt.
-  intros a_in c_in.
-  apply in_bool_In in a_in.
-  apply in_bool_ne_In in c_in.
-  simpl. induction (typs m); simpl in *. destruct a_in.
-  destruct a0. destruct a_in; subst.
-  - rewrite in_app_iff. left. apply c_in.
-  - rewrite in_app_iff. right. apply IHl. auto.
-Qed. 
-
-(*Default def*)
-Definition def_d : def := recursive_def nil.
-
-(*TODO: move*)
-Lemma constr_not_recfun (l: list funpred_def) (f: funsym) 
-  (a: alg_datatype)
-  (m: mut_adt) (l_in: In l (mutfuns_of_context gamma))
-  (m_in: mut_in_ctx m gamma) (a_in: adt_in_mut a m)
-  (f_in1: funsym_in_mutfun f l) (f_in2: constr_in_adt f a):
-  False.
-Proof.
-  destruct gamma_valid as [Hwf _].
-  destruct Hwf as [_ [_[_ [_ [ _ [Hnodup _]]]]]].
-  unfold funsyms_of_context in Hnodup.
-  rewrite NoDup_concat_iff in Hnodup.
-  destruct Hnodup as [_ Hnodup].
-  apply in_bool_In in m_in.
-  unfold funsym_in_mutfun in f_in1.
-  apply in_bool_In in f_in1.
-  pose proof (constr_in_adt_def _ _ _ a_in f_in2) as f_in2'.
-  assert (Hin1: In (recursive_def l) gamma). {
-    apply in_mutfuns_spec. apply l_in.
-  }
-  assert (Hin2: In (datatype_def m) gamma). {
-    apply mut_in_ctx_eq2. apply In_in_bool. apply m_in. 
-  }
-  destruct (In_nth _ _ def_d Hin1) as [i1 [Hi1 Hrecdef]].
-  destruct (In_nth _ _ def_d Hin2) as [i2 [Hi2 Hdatdef]].
-  destruct (Nat.eq_dec i1 i2).
-  - subst. rewrite Hdatdef in Hrecdef. inversion Hrecdef.
-  - apply (Hnodup i1 i2 nil f); try rewrite map_length; auto.
-    rewrite !map_nth_inbound with (d2:=def_d); auto.
-    rewrite Hrecdef, Hdatdef. auto.
-Qed.
-  (*Here, we rely on the fact that we cannot have
-    a funsym that is recursive and also a constructor*)
-Lemma funpred_with_reps_constrs  (pf: pi_funpred gamma_valid pd)
-  (l: list funpred_def)
-  (l_in: In l (mutfuns_of_context gamma)):
-  forall (m : mut_adt) (a : alg_datatype) 
-    (c : funsym) (Hm : mut_in_ctx m gamma) 
-    (Ha : adt_in_mut a m) (Hc : constr_in_adt c a)
-    (srts : list sort)
-    (Hlens : Datatypes.length srts =
-              Datatypes.length (m_params m))
-    (args : arg_list domain
-              (sym_sigma_args c srts)),
-  (funpred_with_reps_funs pf l l_in) c srts args =
-  constr_rep_dom gamma_valid m Hm srts Hlens 
-    (dom_aux pd) a Ha c Hc (Interp.adts pd m srts) args.
-Proof.
-  intros. unfold funpred_with_reps_funs.
-  destruct (funsym_in_mutfun_dec c l);
-  [| destruct pf; apply constrs].
-  destruct (Nat.eq_dec (length srts) (length (s_params c)));
-  [| destruct pf; apply constrs].
-  (*Here, we need a contradiction*)
-  exfalso.
-  apply (constr_not_recfun _ _ _ _ l_in Hm Ha i Hc).
-Qed.
-
-Definition funpred_with_reps (pf: pi_funpred gamma_valid pd)
-(l: list funpred_def)
-(l_in: In l (mutfuns_of_context gamma)):
-pi_funpred gamma_valid pd :=
-Build_pi_funpred gamma_valid pd (funpred_with_reps_funs pf l l_in)
-  (funpred_with_reps_preds pf l l_in)
-  (funpred_with_reps_constrs pf l l_in).
-
-Fixpoint ty_subst' params args (v: vty) : vty :=
-  match v with
-  | vty_int => vty_int
-  | vty_real => vty_real
-  | vty_var x => if in_dec typevar_eq_dec x params then
-    (ty_subst params args) (vty_var x) else vty_var x
-  | vty_cons ts vs =>
-    vty_cons ts (map (ty_subst' params args) vs)
-  end.
-
-(*Get new valuation for [vt_with_args]*)
-Definition upd_vv_args (vt: val_typevar) (vv: val_vars pd vt)
-  params args:
-  length params = length args ->
-  NoDup params ->
-  val_vars pd (vt_with_args vt params args).
-  unfold val_vars.
-  intros Hlen Hparams. unfold val_vars in vv.
-  (*TODO: separate lemma*)
-  (*Hmm this is not quite true because in var case, v_subst chooses
-    a default instead of leaving as is*)
-  assert (forall (v: vty), v_subst (vt_with_args vt params args) v =
-    v_subst vt (ty_subst' params (sorts_to_tys args) v)). {
-    intros. apply sort_inj. simpl.
-    induction v; simpl; auto.
-    - destruct (in_dec typevar_eq_dec v params).
-      + destruct (In_nth _ _ EmptyString i) as [j [Hj Hv]]; subst.
-        rewrite vt_with_args_nth; auto. unfold ty_subst. simpl.
-        rewrite ty_subst_fun_nth with(s:=s_int);
-        unfold sorts_to_tys; auto; [|rewrite map_length]; auto.
-        rewrite map_nth_inbound with(d2:=s_int); [| rewrite <- Hlen]; auto.
-        rewrite <- subst_is_sort_eq; auto.
-        destruct (nth j args s_int); auto.
-      + rewrite vt_with_args_notin; auto.
-    - f_equal. apply list_eq_ext'; rewrite !map_length; auto.
-      intros n d Hn. rewrite !map_nth_inbound with (d2:=vty_int); auto.
-      rewrite Forall_forall in H. apply H. apply nth_In. auto.
-      rewrite map_length; auto.
-  }
-  intros x. rewrite H.
-  (*Is this a hack? Kind of*) apply (vv 
-    (fst x, (ty_subst' params (sorts_to_tys args) (snd x)))).
-Defined.
-
-Lemma fun_in_mutfun {f args body l}:
-In (fun_def f args body) l->
-funsym_in_mutfun f l.
-Proof.
-  intros. apply In_in_bool. simpl.
-  induction l; simpl; destruct H; subst; auto.
-  left; auto. destruct a; simpl; try right; auto.
-Qed.
-
-Lemma pred_in_mutfun {p args body l}:
-In (pred_def p args body) l->
-predsym_in_mutfun p l.
-Proof.
-  intros. apply In_in_bool. simpl.
-  induction l; simpl; destruct H; subst; auto.
-  left; auto. destruct a; simpl; try right; auto.
-Qed.
-
-Lemma f_body_type {l: list funpred_def}
-  (l_in: In l (mutfuns_of_context gamma))
-  {f: funsym} {args: list vsymbol} {body: term}
-  (f_in: In (fun_def f args body) l):
-  term_has_type sigma body (f_ret f).
-Proof.
-  destruct gamma_valid as [_ Hval].
-  rewrite Forall_forall in Hval.
-  apply in_mutfuns_spec in l_in.
-  specialize (Hval _ l_in). simpl in Hval.
-  unfold funpred_valid_type in Hval.
-  destruct Hval as [Hall _].
-  rewrite Forall_forall in Hall.
-  specialize (Hall _ f_in).
-  simpl in Hall.
-  destruct Hall as [Hty _]. apply Hty.
-Qed.
-
-Lemma p_body_type {l: list funpred_def}
-  (l_in: In l (mutfuns_of_context gamma))
-  {p: predsym} {args: list vsymbol} {body: formula}
-  (p_in: In (pred_def p args body) l):
-  valid_formula sigma body.
-Proof.
-  destruct gamma_valid as [_ Hval].
-  rewrite Forall_forall in Hval.
-  apply in_mutfuns_spec in l_in.
-  specialize (Hval _ l_in). simpl in Hval.
-  unfold funpred_valid_type in Hval.
-  destruct Hval as [Hall _].
-  rewrite Forall_forall in Hall.
-  specialize (Hall _ p_in).
-  simpl in Hall.
-  destruct Hall as [Hty _]. apply Hty.
-Qed.
-
-Lemma vt_with_args_cast vt params srts ty:
-  (forall x, In x (type_vars ty) -> In x params) ->
-  NoDup params ->
-  length srts = length params ->
-  v_subst (vt_with_args vt params srts) ty =
-  ty_subst_s params srts ty.
-Proof.
-  intros. apply v_ty_subst_eq; auto.
-  intros. apply vt_with_args_nth; auto.
-Qed.
-
-Lemma recfun_in_funsyms {f: funsym} {l: list funpred_def}
-  (l_in: In l (mutfuns_of_context gamma))
-  (f_in: funsym_in_mutfun f l):
-  In f (funsyms_of_context gamma).
-Proof.
-  unfold funsyms_of_context. rewrite in_concat.
-  exists (funsyms_of_def (recursive_def l)).
-  split. rewrite in_map_iff. exists (recursive_def l).
-  split; auto. apply in_mutfuns_spec in l_in; auto.
-  apply in_bool_In in f_in. auto.
-Qed.
-
-(*NOTE: really could just require f in funsyms_of_context gamma*)
-Lemma funs_cast vt {f: funsym} {srts}
-  (f_in: In f (funsyms_of_context gamma)):
-  length srts = length (s_params f) ->
-  v_subst (vt_with_args vt (s_params f) srts) (f_ret f) = 
-  funsym_sigma_ret f srts.
-Proof.
-  intros.
-  unfold funsym_sigma_ret.
-  apply vt_with_args_cast; auto.
-  2: apply s_params_Nodup.
-  destruct gamma_valid as [Hwf _].
-  destruct Hwf as [Hwf [_ [Hfin _]]].
-  rewrite Forall_forall in Hfin.
-  specialize (Hfin _ f_in).
-  destruct Hwf as [Hwff _].
-  rewrite Forall_forall in Hwff.
-  specialize (Hwff _ Hfin). rewrite Forall_forall in Hwff.
-  specialize (Hwff (f_ret f) (ltac:(simpl; auto))).
-  destruct Hwff as [_ Hall].
-  rewrite Forall_forall in Hall. apply Hall.
-Qed.
-
-(*TODO: move*)
-Lemma funpred_with_reps_funs_notin {pf} {l: list funpred_def}
-  (l_in: In l (mutfuns_of_context gamma))
-  (il: list nat)
-  : length l = length il ->
-forall (f : funsym) (srts : list sort) (a : arg_list domain (sym_sigma_args f srts)),
-~
-In f
-  (map fn_sym
-     (map
-        (fun x : funsym * list vsymbol * term * nat =>
-         fundef_to_fn (fst (fst (fst x))) (snd (fst (fst x))) (snd (fst x)) (snd x))
-        (combine (fst (split_funpred_defs l))
-           (firstn (Datatypes.length (fst (split_funpred_defs l))) 
-           il)))) ->
-funs gamma_valid pd pf f srts a =
-funs gamma_valid pd (funpred_with_reps pf l l_in) f srts a.
-Proof.
-  intros. simpl.
-  unfold funpred_with_reps_funs.
-  destruct (funsym_in_mutfun_dec f l); auto.
-  destruct (Nat.eq_dec (length srts) (length (s_params f))); auto.
-  (*Here is the contradiction*)
-  exfalso.
-  destruct (get_funsym_fn l_in i H) as [f' [Hinf' Hf]]; subst.
-  apply H0. rewrite in_map_iff. exists f'. split; auto.
-Qed.
-
-Lemma funpred_with_reps_preds_notin {pf} {l: list funpred_def}
-  (l_in: In l (mutfuns_of_context gamma))
-  (il: list nat)
-  : length l = length il ->
-  forall (p : predsym) (srts : list sort) (a : arg_list domain (sym_sigma_args p srts)),
-  ~
-  In p
-    (map pn_sym
-       (map
-          (fun x : predsym * list vsymbol * formula * nat =>
-           preddef_to_pn (fst (fst (fst x))) (snd (fst (fst x))) (snd (fst x)) (snd x))
-          (combine (snd (split_funpred_defs l))
-             (skipn (Datatypes.length (fst (split_funpred_defs l))) il)))) ->
-  preds gamma_valid pd pf p srts a =
-  preds gamma_valid pd (funpred_with_reps pf l l_in) p srts a.
-Proof.
-  intros. simpl.
-  unfold funpred_with_reps_preds.
-  destruct (predsym_in_mutfun_dec p l); auto.
-  destruct (Nat.eq_dec (length srts) (length (s_params p))); auto.
-  (*Here is the contradiction*)
-  exfalso.
-  destruct (get_predsym_pn l_in i H) as [f' [Hinf' Hf]]; subst.
-  apply H0. rewrite in_map_iff. exists f'. split; auto.
-Qed.
-
-Lemma vt_with_args_in_eq (ty: vty) (vt1 vt2: val_typevar)
-  params srts:
-  length params = length srts ->
-  NoDup params ->
-  (forall x, In x (type_vars ty) -> In x params) ->
-  v_subst (vt_with_args vt1 params srts) ty =
-  v_subst (vt_with_args vt2 params srts) ty.
-Proof.
-  intros.
-  apply v_subst_ext.
-  intros.
-  apply H1 in H2.
-  destruct (In_nth _ _ EmptyString H2) as [i [Hi Hx]]; subst.
-  rewrite !vt_with_args_nth; auto.
-Qed.
-
-(*Now, we can state our spec:*)
-Theorem funs_rep_spec (pf: pi_funpred gamma_valid pd)
-  (l: list funpred_def)
-  (l_in: In l (mutfuns_of_context gamma)):
-  forall (f: funsym) (args: list vsymbol) (body: term)
-  (f_in: In (fun_def f args body) l)
-  (srts: list sort) (srts_len: length srts = length (s_params f))
-  (a: arg_list domain (sym_sigma_args f srts))
-  (vt: val_typevar) (vv: val_vars pd vt),
-  funs_rep pf f l (fun_in_mutfun f_in) l_in srts srts_len a =
-  (*We need a cast because we change [val_typevar]*)
-  dom_cast _ (funs_cast vt (recfun_in_funsyms l_in (fun_in_mutfun f_in)) srts_len) (
-  (*The function is the same as evaluating the body*)
-  term_rep gamma_valid pd all_unif 
-  (*Setting the function params to srts*)
-  (vt_with_args vt (s_params f) srts)
-  (*And recursively using [funs_rep] and [preds_rep]*)
-  (funpred_with_reps pf l l_in)
-  (*And setting the function arguments to a*)
-  (val_with_args _ _ (upd_vv_args vt vv (s_params f) srts (eq_sym srts_len)
-    (s_params_Nodup _)) args a)
-  (*Evaluating the function body*)
-  body (f_ret f) (f_body_type l_in f_in)).
-Proof.
-  intros.
-  unfold funs_rep. simpl.
-  destruct (funpred_def_valid l l_in) as [Hallval Hex].
-  destruct (Typechecker.funpred_def_term_decide sigma gamma (proj1 gamma_valid) l l_in Hex) as [t Ht].
-  unfold funpred_def_term in Ht.
-  destruct Ht as [Hnotnil [Hlenparams [m_in [Hlen [Hidx [Hfvty [Hpvty [Hfparams [Hpparams [Hfdec Hpdec]]]]]]]]]].
-  (*First step: use [funpred_with_args pf l l_in] instead of pf.
-    we are allowed to do this by [funcs_rep_aux_change_pf]*)
-  unfold funs_rep_aux. simpl.
-  rewrite funcs_rep_aux_change_pf with (pf2:=(funpred_with_reps pf l l_in)).
-  2: {
-    apply funpred_with_reps_funs_notin. auto.
-  }
-  2: { apply funpred_with_reps_preds_notin. auto. }
-
-  (*Simplify f*)
-  assert (Hf: f = fn_sym (proj1_sig (get_funsym_fn l_in (fun_in_mutfun f_in) (eq_sym Hlen)))). {
-    destruct ((get_funsym_fn l_in (fun_in_mutfun f_in) (eq_sym Hlen))); simpl.
-    apply a0.
-  }
-  assert (Hparams: snd (fst (fst t)) = s_params f). {
-    rewrite Hf. 
-    erewrite <- Hfparams. reflexivity.
-    destruct (get_funsym_fn l_in (fun_in_mutfun f_in) (eq_sym Hlen)); simpl.
-    apply a0.
-  }
-  destruct t as [[[m params] vs] il]. simpl in *.
-  generalize dependent ((get_funsym_fn l_in (fun_in_mutfun f_in) (eq_sym Hlen))).
-  intros [f' [Hinf' Hf1]] Hf2. subst. clear Hf2.
-  simpl.
-  (*Now our pf's are the same, so we use [funpred_rep_aux_eq]*)
-  (*TODO: find which vv to use*)
-  erewrite funpred_rep_aux_eq. simpl.
-  - rewrite !dom_cast_compose.
-    (*Now, need to deal with all the casting*) 
-(*So we need to know that (v_subst (vt_with_args triv_val_typevar params srts) ty =
-  v_subst (vt_with_args vt params srts) ty)*)
-assert (Hv: (v_subst (vt_with_args vt (s_params (fn_sym f')) srts) (f_ret (fn_sym f'))) =
-(v_subst (vt_with_args triv_val_typevar (s_params (fn_sym f')) srts)
-(f_ret (fn_sym f')))).
-{
-  apply vt_with_args_in_eq; auto.
-  apply s_params_Nodup.
-  intros x Hinx.
-  apply (@funpred_defs_to_sns_typevars1 l il) with(f:=f')(ty:=(f_ret (fn_sym f')));
-  auto. simpl; auto.
-}
-(*Now these are the same type*)
-match goal with
-| |- dom_cast ?d ?H1 ?t1 = dom_cast ?d ?H2 ?t2 =>
-  assert (t1 = dom_cast (dom_aux pd) Hv t2)
-end.
-2: {
-  rewrite H.
-  rewrite !dom_cast_compose.
-  apply dom_cast_eq.
-}
-(*Ok, now we need to prove this*)
-(*First, simplify cast*)
-unfold cast_arg_list. rewrite !eq_trans_refl_l.
-rewrite !scast_scast. rewrite <- !eq_sym_map_distr.
-rewrite eq_trans_sym_inv_r.
-(*Now we need to transform these, since they use
-  different [val_typevar]s. We use [vt_fv_agree_tm]*)
-assert (body = fn_body f'). {
-  admit.
-}
-assert (args = sn_args f') by admit.
-subst.
-rewrite (term_rep_irrel) with(Hty2:=f_body_type l_in f_in).
-apply vt_fv_agree_tm.
-+ intros x Hinx.
-  (*TODO: require in typing that tm_type_vars body is a
-    subset of params (or s_params)*)
-  assert (In x (s_params (fn_sym f'))) by admit.
-  destruct (In_nth _ _ EmptyString H) as [i [Hi Hx]]; subst.
-  rewrite !vt_with_args_nth; auto; apply s_params_Nodup.
-+ intros x Hinx Heq.
-  (*Here, we prove that the valuations for all free vars
-    are equal*)
-  (*Should have: all free vars are in args - can prove, TODO*)
-  assert (In x (sn_args f')) by admit.
-  destruct (In_nth _ _ vs_d H) as [i [ Hi Hx]]; subst.
-  assert (Hargs: s_args (fn_sym f') = map snd (sn_args f')). {
-    rewrite Forall_forall in Hallval; apply Hallval in f_in.
-    simpl in f_in. symmetry. apply f_in.
-  }
-  assert (Heq1: forall vt, nth i (sym_sigma_args (fn_sym f') srts) s_int =
-  v_subst (vt_with_args vt (s_params (fn_sym f')) srts) (snd (nth i (sn_args f') vs_d))). {
-    intros vt1.
-    unfold sym_sigma_args.  unfold ty_subst_list_s.
-    rewrite map_nth_inbound with(d2:=vty_int); [| rewrite Hargs, map_length; auto].
-    erewrite <- vt_with_args_cast with(vt:=vt1); auto.
-    - rewrite Hargs. rewrite map_nth_inbound with(d2:=vs_d); auto.
-    - intros. 
-      apply (@funpred_defs_to_sns_typevars1 l il) with(f:=f')(ty:=(nth i (s_args (fn_sym f')) vty_int));
-      auto. simpl; auto. right.
-      apply nth_In. rewrite Hargs, map_length; auto.
-    - apply s_params_Nodup.
-  }
-  rewrite val_with_args_in with (Heq:=Heq1 vt); auto.
-  (*TODO: other goals*)
-  2: {
-    rewrite Forall_forall in Hallval. apply Hallval in f_in.
-    simpl in f_in. destruct_all. apply NoDup_map_inv in H2; auto. 
-  }
-  2: {
-    unfold sym_sigma_args, ty_subst_list_s.
-    rewrite map_length, Hargs, map_length.
-    reflexivity.
-  }
-  (*Now we need to rewrite the other one*)
-  rewrite val_with_args_in with(Heq:=Heq1 triv_val_typevar); auto.
-  (*TODO: separate out*)
-  2: {
-    rewrite Forall_forall in Hallval. apply Hallval in f_in.
-    simpl in f_in. destruct_all. apply NoDup_map_inv in H2; auto. 
-  }
-  2: {
-    unfold sym_sigma_args, ty_subst_list_s.
-    rewrite map_length, Hargs, map_length.
-    reflexivity.
-  }
-  rewrite !dom_cast_compose.
-  simpl. apply dom_cast_eq.
-- (*Now we have to prove that the function values are correct*)
-  (*TODO: should be separate lemma*)
-  intros. simpl.
-  unfold funpred_with_reps_funs.
-  destruct (funsym_in_mutfun_dec (fn_sym f) l).
-  + destruct (Nat.eq_dec (Datatypes.length srts0) (Datatypes.length (s_params (fn_sym f)))).
-    * unfold funs_rep. simpl.
-      destruct (funpred_def_valid l l_in) as [Hallval' Hex'].
-      destruct (Typechecker.funpred_def_term_decide sigma gamma (proj1 gamma_valid) l l_in Hex') as [t1 Ht1].
-      unfold funpred_def_term in Ht1.
-      destruct Ht1 as [Hnotnil1 [Hlenparams1 [m_in1 [Hlen1 [Hidx1 [Hfvty1 [Hpvty1 [Hfparams1 [Hpparams1 [Hfdec1 Hpdec1]]]]]]]]]].
-      simpl.
-      assert (Hf: f = (proj1_sig (get_funsym_fn l_in i (eq_sym Hlen1)))). {
-        destruct ((get_funsym_fn l_in i (eq_sym Hlen1))); simpl.
-        (*Use uniqueness*)
-        destruct a1.
-        (*Ugh, the does follow but it is annoying*)
-        admit.
-      }
-      (*TODO: start here (then go back and prove admitted)*)
-
-      (*
-      clear f_in0.
-      assert (Hparams: snd (fst (fst t1)) = s_params f). {
-        rewrite Hf. 
-        erewrite <- Hfparams. reflexivity.
-        destruct (get_funsym_fn l_in (fun_in_mutfun f_in) (eq_sym Hlen)); simpl.
-        apply a0.
-      }
-      destruct t as [[[m params] vs] il]. simpl in *.
-      generalize dependent ((get_funsym_fn l_in (fun_in_mutfun f_in) (eq_sym Hlen))).
-      intros [f' [Hinf' Hf1]] Hf2. subst. clear Hf2.
-      simpl.
-      subst.
-      generalize dependent ((get_funsym_fn l_in i (eq_sym Hlen1))).
-      intros [f'' [Hinf'' Hf2]] Hf3. subst. clear Hf3.
-      simpl.
-      assert ()
-      Check (f_equal (fun x : funsym => funsym_sigma_ret x srts0)
-      (eq_sym (proj2 (conj Hinf'' Hf2)))).
-      Check (f_equal (fun x : funsym => funsym_sigma_ret x srts0)
-      (eq_sym (proj2 (proj2_sig (get_funsym_fn l_in i (eq_sym Hlen1)))))).
-      Check (f_equal (fun x : funsym => funsym_sigma_ret x srts0)
-      (eq_sym (proj2 (proj2_sig (get_funsym_fn l_in i (eq_sym Hlen1)))))).
-
-
-  unfold funpred_with_reps.
-   simpl.
-  unfold funs_rep_aux.
-  Unshelve.
-  [| apply s_params_Nodup|].
-  Unshelve.
-  Search val_with_args.
-
-
-  val_with_args_in:
-  forall {pd : pi_dom} (m : mut_adt) (vs : list vty),
-  Datatypes.length vs = Datatypes.length (m_params m) ->
-  forall (vt : val_typevar) (vv : val_vars pd vt) 
-	(vars : list vsymbol) (srts : list sort)
-    (a : arg_list (IndTypes.domain (dom_aux pd)) srts),
-  NoDup vars ->
-  Datatypes.length vars = Datatypes.length srts ->
-  forall i : nat,
-  i < Datatypes.length vars ->
-  forall Heq : nth i srts s_int = v_subst vt (snd (nth i vars vs_d)),
-  val_with_args vt vv vars a (nth i vars vs_d) =
-  dom_cast (dom_aux pd) Heq (hnth i a s_int (dom_int pd))
-
-
-
-
-(*Now we show that the valuation*)
-
-Search eq_trans eq_sym.
-Search f_equal eq_sym.
-rewrite !eq_trans_map_distr.
-Search eq_trans f_equal.
-
-unfold proj2.
-
-
-simpl.
-
-vt_with_args_in_eq
-
-  
-  unfold funs_rep_aux.
-  (*TODO: need to prove, rewrite with other pf first*)
-  erewrite funpred_rep_aux_eq. simpl.
-  Search funs_rep_aux.
-  simpl.*)
-Admitted.
-
-(*The pred spec is easier, we don't need a cast*)
-Theorem preds_rep_spec (pf: pi_funpred gamma_valid pd)
-  (l: list funpred_def)
-  (l_in: In l (mutfuns_of_context gamma)):
-  forall (p: predsym) (args: list vsymbol) (body: formula)
-  (p_in: In (pred_def p args body) l)
-  (srts: list sort) (srts_len: length srts = length (s_params p))
-  (a: arg_list domain (sym_sigma_args p srts))
-  (vt: val_typevar) (vv: val_vars pd vt),
-  preds_rep pf p l (pred_in_mutfun p_in) l_in srts srts_len a =
-  (*The function is the same as evaluating the body*)
-  formula_rep gamma_valid pd all_unif 
-  (*Setting the function params to srts*)
-  (vt_with_args vt (s_params p) srts)
-  (*And recursively using [funs_rep] and [preds_rep]*)
-  (funpred_with_reps pf l l_in)
-  (*And setting the function arguments to a*)
-  (val_with_args _ _ (upd_vv_args vt vv (s_params p) srts (eq_sym srts_len)
-    (s_params_Nodup _)) args a)
-  (*Evaluating the function body*)
-  body (p_body_type l_in p_in).
-Proof.
-Admitted.
-
-
-End Full.
