proofs/core/RecFun2.v
@@ -1,0 +1,1034 @@
+Require Export RecFun.
+
+(*This gives the full definition and spec for recursive
+  functions, given a well-typed context and a function definition
+  in this context. We separate it from the core definitions (RecFun.v)
+  because those are very large, complicated, and ugly, and 
+  they take a very long to compile*)
+
+(*Now we give the full definition*)
+Section Full.
+
+(*First, we define when a mutual function body is in a context*)
+
+(*TODO: move*)
+
+(*Similar to mutual types*)
+
+Definition funsym_in_mutfun (f: funsym) (l: list funpred_def) : bool :=
+  in_bool funsym_eq_dec f (funsyms_of_def (recursive_def l)).
+
+Definition get_mutfun_fun (f: funsym) (gamma': context) : option (list funpred_def) :=
+  find (funsym_in_mutfun f) (mutfuns_of_context gamma').
+
+Definition predsym_in_mutfun (p: predsym) (l: list funpred_def) : bool :=
+  in_bool predsym_eq_dec p (predsyms_of_def (recursive_def l)).
+
+Definition get_mutfun_pred (p: predsym) (gamma': context) : option (list funpred_def) :=
+  find (predsym_in_mutfun p) (mutfuns_of_context gamma').
+
+
+
+Context {sigma: sig} {gamma: context} (gamma_valid: valid_context sigma gamma)
+{pd: pi_dom} (all_unif: forall m, mut_in_ctx m gamma -> IndTypes.uniform m).
+
+
+
+(*TODO: move to typing*)
+
+Lemma funpred_def_valid (l: list funpred_def)
+  (l_in: In l (mutfuns_of_context gamma)):
+  funpred_valid_type sigma gamma l.
+Proof.
+  destruct gamma_valid.
+  rewrite Forall_forall in H0.
+  rewrite in_mutfuns_spec in l_in.
+  specialize (H0 _ l_in). exact H0.
+Qed.
+
+Lemma funpred_defs_to_sns_types l il:
+  length l = length il ->
+  In l (mutfuns_of_context gamma) ->
+  Forall (fun f => term_has_type sigma (fn_body f) (f_ret (fn_sym f))) 
+    (fst (funpred_defs_to_sns l il)).
+Proof.
+  intros. apply funpred_def_valid in H0.
+  unfold funpred_valid_type in H0.
+  destruct H0.
+  rewrite Forall_forall.
+  intros x. rewrite funpred_defs_to_sns_in_fst; auto.
+  intros [i [Hi Hx]].
+  rewrite Forall_forall in H0.
+  set (y:=nth i (fst (split_funpred_defs l)) (id_fs, [], tm_d)) in *.
+  simpl in Hx.
+  subst. 
+  assert (In (fun_def (fst (fst y)) (snd (fst y)) (snd y)) l). {
+    apply (split_funpred_defs_in_l l). subst y. apply nth_In. auto.
+  }
+  apply H0 in H2. simpl in H2.
+  destruct_all. unfold well_typed_term in H2.
+  destruct H2.
+  simpl. apply H2.
+Qed.
+
+Lemma funpred_defs_to_sns_valid l il:
+  length l = length il ->
+  In l (mutfuns_of_context gamma) ->
+  Forall (fun p => valid_formula sigma (pn_body p)) 
+    (snd (funpred_defs_to_sns l il)).
+Proof.
+  intros. apply funpred_def_valid in H0.
+  unfold funpred_valid_type in H0.
+  destruct H0.
+  rewrite Forall_forall.
+  intros x. rewrite funpred_defs_to_sns_in_snd; auto.
+  intros [i [Hi Hx]].
+  rewrite Forall_forall in H0.
+  set (y:=nth i (snd (split_funpred_defs l)) (id_ps, [], Ftrue)) in *.
+  simpl in Hx.
+  subst. simpl. 
+  assert (In (pred_def (fst (fst y)) (snd (fst y)) (snd y)) l). {
+    apply (split_funpred_defs_in_l l). subst y. apply nth_In. auto.
+  }
+  apply H0 in H2. simpl in H2.
+  destruct_all. unfold well_typed_term in H2.
+  destruct H2. auto.
+Qed.
+
+(*Prove the typevar condition
+  This proof is annoying because there is so much unfolding
+  and proving equivalences between being "in" different lists,
+  but it it not too hard*)
+Lemma funpred_defs_to_sns_typevars1 {l: list funpred_def} 
+  {il: list nat} {params: list typevar}
+  (l_in: In l (mutfuns_of_context gamma))
+  (Hparams: forall f : fn,
+    In f (fst (funpred_defs_to_sns l il)) ->
+    s_params (fn_sym f) = params):
+  length l = length il ->
+  (forall f : fn,
+  In f (fst (funpred_defs_to_sns l il)) ->
+  forall ty : vty,
+  In ty (f_ret (fn_sym f) :: s_args (fn_sym f)) ->
+  forall x : typevar, In x (type_vars ty) -> In x params).
+Proof.
+  intros Hlen. intros.
+  destruct gamma_valid as [Hwf _].
+  unfold wf_context in Hwf.
+  destruct Hwf as [Hwf [_ [Hallin _]]].
+  unfold wf_sig in Hwf. destruct Hwf as [Halltyp _].
+  rewrite Forall_forall in Hallin.
+  assert (Hin:=H).
+  rewrite funpred_defs_to_sns_in_fst in H; auto.
+  destruct H as [i [Hi Hf]].
+  set (y:=nth i (fst (split_funpred_defs l)) (id_fs, [], tm_d)) in *.
+  simpl in Hf.
+  subst. simpl in H0.
+  assert (In (fun_def (fst (fst y)) (snd (fst y)) (snd y)) l). {
+    apply (split_funpred_defs_in_l l). subst y. apply nth_In. auto.
+  }
+  assert (Hinf: In (fst (fst y)) (funsyms_of_context gamma)). {
+    unfold funsyms_of_context. rewrite in_concat.
+    exists (funsyms_of_def (recursive_def l)). split; auto.
+    rewrite in_map_iff. exists (recursive_def l); split; auto.
+    apply in_mutfuns_spec; auto.
+    clear -H. generalize dependent y; intros.
+    simpl. induction l; simpl; [inversion H |]. destruct a; simpl; auto;
+    destruct H; simpl; auto; inversion H; subst; auto.
+  }
+  specialize (Hallin _ Hinf).
+  rewrite Forall_forall in Halltyp.
+  specialize (Halltyp _ Hallin).
+  rewrite Forall_forall in Halltyp.
+  specialize (Halltyp ty H0). destruct Halltyp as [Hvalty Hallty].
+  rewrite Forall_forall in Hallty.
+  rewrite <- (Hparams _ Hin). simpl. apply Hallty. auto.
+Qed.
+
+Lemma funpred_defs_to_sns_typevars2 {l: list funpred_def} 
+  {il: list nat} {params: list typevar}
+  (l_in: In l (mutfuns_of_context gamma))
+  (Hparams: forall p : pn,
+    In p (snd (funpred_defs_to_sns l il)) ->
+    s_params (pn_sym p) = params):
+  length l = length il ->
+  (forall p : pn,
+  In p (snd (funpred_defs_to_sns l il)) ->
+  forall ty : vty,
+  In ty (s_args (pn_sym p)) ->
+  forall x : typevar, In x (type_vars ty) -> In x params).
+Proof.
+  intros Hlen. intros.
+  destruct gamma_valid as [Hwf _].
+  unfold wf_context in Hwf.
+  destruct Hwf as [Hwf [_ [_ [Hallin _]]]].
+  unfold wf_sig in Hwf. destruct Hwf as [_ Halltyp].
+  rewrite Forall_forall in Hallin.
+  assert (Hin:=H).
+  rewrite funpred_defs_to_sns_in_snd in H; auto.
+  destruct H as [i [Hi Hf]].
+  set (y:=nth i (snd (split_funpred_defs l)) (id_ps, [], Ftrue)) in *.
+  simpl in Hf.
+  rewrite map_length in Hf.
+  replace (length (combine (fst (split_funpred_defs l))
+  (firstn (Datatypes.length (fst (split_funpred_defs l))) il))) with
+  (length (fst (split_funpred_defs l))) in Hf by
+    (rewrite combine_length, firstn_length;
+    pose proof (split_funpred_defs_length l); lia).
+  subst. simpl in H0.
+  assert (In (pred_def (fst (fst y)) (snd (fst y)) (snd y)) l). {
+    apply (split_funpred_defs_in_l l). subst y. apply nth_In. auto.
+  }
+  assert (Hinf: In (fst (fst y)) (predsyms_of_context gamma)). {
+    unfold predsyms_of_context. rewrite in_concat.
+    exists (predsyms_of_def (recursive_def l)). split; auto.
+    rewrite in_map_iff. exists (recursive_def l); split; auto.
+    apply in_mutfuns_spec; auto.
+    clear -H. generalize dependent y; intros.
+    simpl. induction l; simpl; [inversion H |]. destruct a; simpl; auto;
+    destruct H; simpl; auto; inversion H; subst; auto.
+  }
+  specialize (Hallin _ Hinf).
+  rewrite Forall_forall in Halltyp.
+  specialize (Halltyp _ Hallin).
+  rewrite Forall_forall in Halltyp.
+  specialize (Halltyp ty H0). destruct Halltyp as [Hvalty Hallty].
+  rewrite Forall_forall in Hallty.
+  rewrite <- (Hparams _ Hin). simpl. apply Hallty. auto.
+Qed.
+
+Lemma get_funsym_fn {l: list funpred_def} {il} {f: funsym}
+  (l_in: In l (mutfuns_of_context gamma))
+  (f_in: funsym_in_mutfun f l):
+  length l = length il ->
+  { f' : fn | In f' (fst (funpred_defs_to_sns l il)) /\ 
+    f = fn_sym f' }.
+Proof.
+  intros.
+  destruct (find_fn f (fst (funpred_defs_to_sns l il))); auto.
+  (*Just need to show contradiction case - we can use Props here*)
+  exfalso.
+  apply n.
+  clear n.
+  apply in_bool_In in f_in.
+  assert ((fold_right
+  (fun (x : funpred_def) (acc : list funsym) =>
+   match x with
+   | fun_def f' _ _ => f' :: acc
+   | pred_def _ _ _ => acc
+   end) [] l) = (map fn_sym (fst (funpred_defs_to_sns l il)))). {
+    unfold funpred_defs_to_sns; simpl.
+    pose proof (split_funpred_defs_length l).
+    rewrite !map_map. simpl. rewrite map_fst_fst_fst_combine by
+      (rewrite firstn_length; lia).
+    clear. induction l; simpl; auto; destruct a; simpl; auto.
+    f_equal; auto.
+  }
+  rewrite <- H0; auto.
+Qed.
+
+Lemma get_predsym_pn {l: list funpred_def} {il} {p: predsym}
+  (l_in: In l (mutfuns_of_context gamma))
+  (p_in: predsym_in_mutfun p l):
+  length l = length il ->
+  { p' : pn | In p' (snd (funpred_defs_to_sns l il)) /\ 
+    p = pn_sym p' }.
+Proof.
+  intros.
+  destruct (find_pn p (snd (funpred_defs_to_sns l il))); auto.
+  (*Just need to show contradiction case - we can use Props here*)
+  exfalso.
+  apply n.
+  clear n.
+  apply in_bool_In in p_in.
+  assert ((fold_right
+  (fun (x : funpred_def) (acc : list predsym) =>
+   match x with
+   | fun_def _ _ _ => acc
+   | pred_def p' _ _ => p' :: acc
+   end) [] l) = (map pn_sym (snd (funpred_defs_to_sns l il)))). {
+    unfold funpred_defs_to_sns; simpl.
+    pose proof (split_funpred_defs_length l).
+    rewrite !map_map. simpl. rewrite map_fst_fst_fst_combine by
+      (rewrite skipn_length; lia).
+    clear. induction l; simpl; auto; destruct a; simpl; auto.
+    f_equal; auto.
+  }
+  rewrite <- H0; auto.
+Qed.
+
+(*Get fs and ps associated with a funpred_def*)
+Definition get_funpred_def_info (l: list funpred_def)
+  (l_in: In l (mutfuns_of_context gamma)):
+  (list fn * list pn).
+Proof.
+  pose proof (funpred_def_valid _ l_in) as Hval.
+  unfold funpred_valid_type in Hval.
+  destruct Hval.
+  (*Here, we use the typechecking result that it is
+    decidable to find the list of indices*)
+  apply (Typechecker.funpred_def_term_decide sigma gamma (proj1 gamma_valid) _ l_in) 
+  in H0.
+  destruct H0 as [t Ht].
+  exact (funpred_defs_to_sns l (snd t)).
+Defined.
+
+(*We will need to prove that this has all of the desired properties*)
+
+
+Notation domain := (domain (dom_aux pd)).
+
+(*Here, we fix our valuation since we cannot take in any
+  input in our final version. We can give a trivial valuation
+  and define the mapping on the typesyms and vsyms that we care
+  about. We will need to show it equals a [term_rep] and [formula_rep]
+  for an arbirtary valuation, which will require a bit of annoying casting*)
+
+
+(*Definition of funs_rep - what we will set each recursive function
+  to in our full interp.
+  The difficulty in defining this is in showing that all of the
+  conditions we need about fs and ps are satisfied; they
+  all follow, in one way or another, from the wf context and/or
+  the typechecker's correctness.
+  We need a pf to know how to evaluate other function and
+  predicate symbols (non-recursive ones)*)
+Definition funs_rep (pf: pi_funpred gamma_valid pd) 
+  (f: funsym) (l: list funpred_def)
+  (f_in: funsym_in_mutfun f l)
+  (l_in: In l (mutfuns_of_context gamma))
+  (srts: list sort)
+  (srts_len: length srts = length (s_params f))
+  (a: arg_list domain (sym_sigma_args f srts)):
+  domain (funsym_sigma_ret f srts).
+(*TODO: manual definition?*)
+Proof.
+  pose proof (funpred_def_valid _ l_in) as Hval.
+  destruct Hval as [Hval Hex].
+  apply (Typechecker.funpred_def_term_decide sigma gamma (proj1 gamma_valid) _ l_in) 
+  in Hex.
+  destruct Hex as [t Ht].
+  set (sns := (funpred_defs_to_sns l (snd t))).
+  unfold funpred_def_term in Ht.
+  destruct Ht as [Hnotnil [Hlenparams [m_in [Hlen [Hidx [Hfvty [Hpvty [Hfparams [Hpparams [Hfdec Hpdec]]]]]]]]]].
+  set (vt:=(vt_with_args triv_val_typevar (snd (fst (fst t))) srts)).
+  set (fn_info := get_funsym_fn l_in f_in (eq_sym Hlen)).
+  assert (Hsrtslen': Datatypes.length srts = Datatypes.length (snd (fst (fst t)))). {
+    rewrite srts_len, (proj2' (proj2_sig fn_info)), 
+    (Hfparams _ (proj1' (proj2_sig fn_info))).
+    reflexivity.
+  }
+  assert (Hparamsnodup: NoDup (snd (fst (fst t)))). {
+    rewrite <- (Hfparams _ (proj1' (proj2_sig fn_info))).
+    apply s_params_Nodup.
+  }
+  set (Heqf :=
+  eq_trans (f_equal f_sym (proj2' (proj2_sig fn_info)))
+  (fs_wf_eq _ (proj1' (funpred_def_to_sns_wf sigma gamma l (snd t) Hlen Hidx Hval))
+  _ (proj1' (proj2_sig fn_info))) : f_sym f = sn_sym (proj1_sig fn_info) ).
+  set (a':= (cast_arg_list (f_equal (fun x => sym_sigma_args x srts) Heqf) a)).
+  (*Need to get the fn associated with this funsym*)
+  (*We call [funs_rep_aux] with all of the proofs we need; we need
+    to cast the result because it returns something basedon the funsym*)
+  exact (dom_cast _ 
+    (f_equal (fun x => funsym_sigma_ret x srts) (eq_sym (proj2 (proj2_sig fn_info))))
+
+  (@funs_rep_aux _ _ gamma_valid pd all_unif (fst sns) (snd sns)
+    (proj1' (funpred_def_to_sns_wf sigma gamma l (snd t) Hlen Hidx Hval))
+    (proj2' (funpred_def_to_sns_wf sigma gamma l (snd t) Hlen Hidx Hval))
+    (proj1' (funpred_defs_to_sns_NoDup (proj1 gamma_valid) _ _ l_in (eq_sym Hlen)))
+    (proj2' (funpred_defs_to_sns_NoDup (proj1 gamma_valid) _ _ l_in (eq_sym Hlen)))
+    (funpred_defs_to_sns_types _ _ (eq_sym Hlen) l_in)
+    (funpred_defs_to_sns_valid _ _ (eq_sym Hlen) l_in)
+    (snd (fst (fst t))) Hfparams Hpparams
+    (funpred_defs_to_sns_typevars1 l_in Hfparams (eq_sym Hlen))
+    (funpred_defs_to_sns_typevars2 l_in Hpparams (eq_sym Hlen))
+    (fst (fst (fst t))) (snd (fst t)) Hlenparams Hfvty Hpvty Hfdec Hpdec 
+      m_in (*pf*) _ pf (triv_val_vars pd vt)
+    (proj1_sig fn_info)
+    (proj1' (proj2_sig fn_info))
+    srts Hsrtslen'
+    (vt_with_args_vt_eq _ _ Hparamsnodup Hsrtslen')
+    a')).
+Defined.
+
+(*preds_rep*)
+Definition preds_rep (pf: pi_funpred gamma_valid pd) 
+  (p: predsym) (l: list funpred_def)
+  (p_in: predsym_in_mutfun p l)
+  (l_in: In l (mutfuns_of_context gamma))
+  (srts: list sort)
+  (srts_len: length srts = length (s_params p))
+  (a: arg_list domain (sym_sigma_args p srts)):
+  bool.
+(*TODO: manual definition?*)
+Proof.
+  pose proof (funpred_def_valid _ l_in) as Hval.
+  destruct Hval as [Hval Hex].
+  apply (Typechecker.funpred_def_term_decide sigma gamma (proj1 gamma_valid) _ l_in) 
+  in Hex.
+  destruct Hex as [t Ht].
+  set (sns := (funpred_defs_to_sns l (snd t))).
+  unfold funpred_def_term in Ht.
+  destruct Ht as [Hnotnil [Hlenparams [m_in [Hlen [Hidx [Hfvty [Hpvty [Hfparams [Hpparams [Hfdec Hpdec]]]]]]]]]].
+  set (vt:=(vt_with_args triv_val_typevar (snd (fst (fst t))) srts)).
+  set (pn_info := get_predsym_pn l_in p_in (eq_sym Hlen)).
+  assert (Hsrtslen': Datatypes.length srts = Datatypes.length (snd (fst (fst t)))). {
+    rewrite srts_len, (proj2 (proj2_sig pn_info)), 
+    (Hpparams _ (proj1 (proj2_sig pn_info))).
+    reflexivity.
+  }
+  assert (Hparamsnodup: NoDup (snd (fst (fst t)))). {
+    rewrite <- (Hpparams _ (proj1 (proj2_sig pn_info))).
+    apply s_params_Nodup.
+  }
+  set (Heqf :=
+  eq_trans (f_equal p_sym (proj2 (proj2_sig pn_info)))
+  (ps_wf_eq _ (proj2 (funpred_def_to_sns_wf sigma gamma l (snd t) Hlen Hidx Hval))
+  _ (proj1 (proj2_sig pn_info))) : p_sym p = sn_sym (proj1_sig pn_info) ).
+  set (a':= (cast_arg_list (f_equal (fun x => sym_sigma_args x srts) Heqf) a)).
+  (*Need to get the fn associated with this funsym*)
+  (*We call [funs_rep_aux] with all of the proofs we need; we need
+    to cast the result because it returns something basedon the funsym*)
+  exact (@preds_rep_aux _ _ gamma_valid pd all_unif (fst sns) (snd sns)
+    (proj1 (funpred_def_to_sns_wf sigma gamma l (snd t) Hlen Hidx Hval))
+    (proj2 (funpred_def_to_sns_wf sigma gamma l (snd t) Hlen Hidx Hval))
+    (proj1 (funpred_defs_to_sns_NoDup (proj1 gamma_valid) _ _ l_in (eq_sym Hlen)))
+    (proj2 (funpred_defs_to_sns_NoDup (proj1 gamma_valid) _ _ l_in (eq_sym Hlen)))
+    (funpred_defs_to_sns_types _ _ (eq_sym Hlen) l_in)
+    (funpred_defs_to_sns_valid _ _ (eq_sym Hlen) l_in)
+    (snd (fst (fst t))) Hfparams Hpparams
+    (funpred_defs_to_sns_typevars1 l_in Hfparams (eq_sym Hlen))
+    (funpred_defs_to_sns_typevars2 l_in Hpparams (eq_sym Hlen))
+    (fst (fst (fst t))) (snd (fst t)) Hlenparams Hfvty Hpvty Hfdec Hpdec 
+      m_in _ pf (triv_val_vars pd vt)
+    (proj1_sig pn_info)
+    (proj1 (proj2_sig pn_info))
+    srts Hsrtslen'
+    (vt_with_args_vt_eq _ _ Hparamsnodup Hsrtslen')
+    a').
+Defined.
+
+Lemma funsym_in_mutfun_dec: forall f l, { funsym_in_mutfun f l} + {~ funsym_in_mutfun f l}.
+Proof.
+  intros. destruct (funsym_in_mutfun f l) eqn : Ha. auto. right.
+  intro C; inversion C.
+Qed.
+
+Lemma predsym_in_mutfun_dec: forall p l, { predsym_in_mutfun p l} + 
+  {~ predsym_in_mutfun p l}.
+Proof.
+  intros. destruct (predsym_in_mutfun p l) eqn : Ha. auto. right.
+  intro C; inversion C.
+Qed.
+
+(*Now we define a modified pi_funpred, where we interpret
+  these functions and predicates using their reps*)
+Definition funpred_with_reps_funs (pf: pi_funpred gamma_valid pd)
+  (l: list funpred_def)
+  (l_in: In l (mutfuns_of_context gamma)) :
+  forall (f: funsym) (srts: list sort)
+  (a: arg_list domain (sym_sigma_args f srts)),
+  domain (funsym_sigma_ret f srts) :=
+
+  (*Need to see if f in l and srts has right length*)
+  fun f srts a => 
+    match funsym_in_mutfun_dec f l with (*funsym_in_mutfun f l as b return funsym_in_mutfun f l = b -> 
+      domain (funsym_sigma_ret f srts) *)
+    | left f_in => 
+      (*TODO: should we require srts_len always?*)
+      match (Nat.eq_dec (length srts) (length (s_params f) )) with
+      | left srts_len =>
+        funs_rep pf f l f_in l_in srts srts_len a
+      | right srts_len => (funs gamma_valid pd pf) f srts a
+      end
+    | right f_notin => (funs gamma_valid pd pf) f srts a
+    end.
+
+Definition funpred_with_reps_preds (pf: pi_funpred gamma_valid pd)
+  (l: list funpred_def)
+  (l_in: In l (mutfuns_of_context gamma)) :
+  forall (p: predsym) (srts: list sort)
+  (a: arg_list domain (sym_sigma_args p srts)),
+  bool :=
+
+  (*Need to see if f in l and srts has right length*)
+  fun p srts a => 
+    match predsym_in_mutfun_dec p l with
+    | left p_in =>
+      (*TODO: should we require srts_len always?*)
+      match (Nat.eq_dec (length srts) (length (s_params p) ))with
+      | left srts_len =>
+        preds_rep pf p l p_in l_in srts srts_len a
+      | right srts_len => (preds gamma_valid pd pf) p srts a
+      end
+    | right p_notin => (preds gamma_valid pd pf) p srts a
+    end.
+
+Lemma constr_in_adt_def a m f:
+  adt_in_mut a m ->
+  constr_in_adt f a ->
+  In f (funsyms_of_def (datatype_def m)).
+Proof.
+  unfold mut_in_ctx. unfold adt_in_mut. unfold constr_in_adt.
+  intros a_in c_in.
+  apply in_bool_In in a_in.
+  apply in_bool_ne_In in c_in.
+  simpl. induction (typs m); simpl in *. destruct a_in.
+  destruct a0. destruct a_in; subst.
+  - rewrite in_app_iff. left. apply c_in.
+  - rewrite in_app_iff. right. apply IHl. auto.
+Qed. 
+
+(*Default def*)
+Definition def_d : def := recursive_def nil.
+
+(*TODO: move*)
+Lemma constr_not_recfun (l: list funpred_def) (f: funsym) 
+  (a: alg_datatype)
+  (m: mut_adt) (l_in: In l (mutfuns_of_context gamma))
+  (m_in: mut_in_ctx m gamma) (a_in: adt_in_mut a m)
+  (f_in1: funsym_in_mutfun f l) (f_in2: constr_in_adt f a):
+  False.
+Proof.
+  destruct gamma_valid as [Hwf _].
+  destruct Hwf as [_ [_[_ [_ [ _ [Hnodup _]]]]]].
+  unfold funsyms_of_context in Hnodup.
+  rewrite NoDup_concat_iff in Hnodup.
+  destruct Hnodup as [_ Hnodup].
+  apply in_bool_In in m_in.
+  unfold funsym_in_mutfun in f_in1.
+  apply in_bool_In in f_in1.
+  pose proof (constr_in_adt_def _ _ _ a_in f_in2) as f_in2'.
+  assert (Hin1: In (recursive_def l) gamma). {
+    apply in_mutfuns_spec. apply l_in.
+  }
+  assert (Hin2: In (datatype_def m) gamma). {
+    apply mut_in_ctx_eq2. apply In_in_bool. apply m_in. 
+  }
+  destruct (In_nth _ _ def_d Hin1) as [i1 [Hi1 Hrecdef]].
+  destruct (In_nth _ _ def_d Hin2) as [i2 [Hi2 Hdatdef]].
+  destruct (Nat.eq_dec i1 i2).
+  - subst. rewrite Hdatdef in Hrecdef. inversion Hrecdef.
+  - apply (Hnodup i1 i2 nil f); try rewrite map_length; auto.
+    rewrite !map_nth_inbound with (d2:=def_d); auto.
+    rewrite Hrecdef, Hdatdef. auto.
+Qed.
+  (*Here, we rely on the fact that we cannot have
+    a funsym that is recursive and also a constructor*)
+Lemma funpred_with_reps_constrs  (pf: pi_funpred gamma_valid pd)
+  (l: list funpred_def)
+  (l_in: In l (mutfuns_of_context gamma)):
+  forall (m : mut_adt) (a : alg_datatype) 
+    (c : funsym) (Hm : mut_in_ctx m gamma) 
+    (Ha : adt_in_mut a m) (Hc : constr_in_adt c a)
+    (srts : list sort)
+    (Hlens : Datatypes.length srts =
+              Datatypes.length (m_params m))
+    (args : arg_list domain
+              (sym_sigma_args c srts)),
+  (funpred_with_reps_funs pf l l_in) c srts args =
+  constr_rep_dom gamma_valid m Hm srts Hlens 
+    (dom_aux pd) a Ha c Hc (Interp.adts pd m srts) args.
+Proof.
+  intros. unfold funpred_with_reps_funs.
+  destruct (funsym_in_mutfun_dec c l);
+  [| destruct pf; apply constrs].
+  destruct (Nat.eq_dec (length srts) (length (s_params c)));
+  [| destruct pf; apply constrs].
+  (*Here, we need a contradiction*)
+  exfalso.
+  apply (constr_not_recfun _ _ _ _ l_in Hm Ha i Hc).
+Qed.
+
+Definition funpred_with_reps (pf: pi_funpred gamma_valid pd)
+(l: list funpred_def)
+(l_in: In l (mutfuns_of_context gamma)):
+pi_funpred gamma_valid pd :=
+Build_pi_funpred gamma_valid pd (funpred_with_reps_funs pf l l_in)
+  (funpred_with_reps_preds pf l l_in)
+  (funpred_with_reps_constrs pf l l_in).
+
+Fixpoint ty_subst' params args (v: vty) : vty :=
+  match v with
+  | vty_int => vty_int
+  | vty_real => vty_real
+  | vty_var x => if in_dec typevar_eq_dec x params then
+    (ty_subst params args) (vty_var x) else vty_var x
+  | vty_cons ts vs =>
+    vty_cons ts (map (ty_subst' params args) vs)
+  end.
+
+(*Get new valuation for [vt_with_args]*)
+Definition upd_vv_args (vt: val_typevar) (vv: val_vars pd vt)
+  params args:
+  length params = length args ->
+  NoDup params ->
+  val_vars pd (vt_with_args vt params args).
+  unfold val_vars.
+  intros Hlen Hparams. unfold val_vars in vv.
+  (*TODO: separate lemma*)
+  (*Hmm this is not quite true because in var case, v_subst chooses
+    a default instead of leaving as is*)
+  assert (forall (v: vty), v_subst (vt_with_args vt params args) v =
+    v_subst vt (ty_subst' params (sorts_to_tys args) v)). {
+    intros. apply sort_inj. simpl.
+    induction v; simpl; auto.
+    - destruct (in_dec typevar_eq_dec v params).
+      + destruct (In_nth _ _ EmptyString i) as [j [Hj Hv]]; subst.
+        rewrite vt_with_args_nth; auto. unfold ty_subst. simpl.
+        rewrite ty_subst_fun_nth with(s:=s_int);
+        unfold sorts_to_tys; auto; [|rewrite map_length]; auto.
+        rewrite map_nth_inbound with(d2:=s_int); [| rewrite <- Hlen]; auto.
+        rewrite <- subst_is_sort_eq; auto.
+        destruct (nth j args s_int); auto.
+      + rewrite vt_with_args_notin; auto.
+    - f_equal. apply list_eq_ext'; rewrite !map_length; auto.
+      intros n d Hn. rewrite !map_nth_inbound with (d2:=vty_int); auto.
+      rewrite Forall_forall in H. apply H. apply nth_In. auto.
+      rewrite map_length; auto.
+  }
+  intros x. rewrite H.
+  (*Is this a hack? Kind of*) apply (vv 
+    (fst x, (ty_subst' params (sorts_to_tys args) (snd x)))).
+Defined.
+
+Lemma fun_in_mutfun {f args body l}:
+In (fun_def f args body) l->
+funsym_in_mutfun f l.
+Proof.
+  intros. apply In_in_bool. simpl.
+  induction l; simpl; destruct H; subst; auto.
+  left; auto. destruct a; simpl; try right; auto.
+Qed.
+
+Lemma pred_in_mutfun {p args body l}:
+In (pred_def p args body) l->
+predsym_in_mutfun p l.
+Proof.
+  intros. apply In_in_bool. simpl.
+  induction l; simpl; destruct H; subst; auto.
+  left; auto. destruct a; simpl; try right; auto.
+Qed.
+
+Lemma f_body_type {l: list funpred_def}
+  (l_in: In l (mutfuns_of_context gamma))
+  {f: funsym} {args: list vsymbol} {body: term}
+  (f_in: In (fun_def f args body) l):
+  term_has_type sigma body (f_ret f).
+Proof.
+  destruct gamma_valid as [_ Hval].
+  rewrite Forall_forall in Hval.
+  apply in_mutfuns_spec in l_in.
+  specialize (Hval _ l_in). simpl in Hval.
+  unfold funpred_valid_type in Hval.
+  destruct Hval as [Hall _].
+  rewrite Forall_forall in Hall.
+  specialize (Hall _ f_in).
+  simpl in Hall.
+  destruct Hall as [Hty _]. apply Hty.
+Qed.
+
+Lemma p_body_type {l: list funpred_def}
+  (l_in: In l (mutfuns_of_context gamma))
+  {p: predsym} {args: list vsymbol} {body: formula}
+  (p_in: In (pred_def p args body) l):
+  valid_formula sigma body.
+Proof.
+  destruct gamma_valid as [_ Hval].
+  rewrite Forall_forall in Hval.
+  apply in_mutfuns_spec in l_in.
+  specialize (Hval _ l_in). simpl in Hval.
+  unfold funpred_valid_type in Hval.
+  destruct Hval as [Hall _].
+  rewrite Forall_forall in Hall.
+  specialize (Hall _ p_in).
+  simpl in Hall.
+  destruct Hall as [Hty _]. apply Hty.
+Qed.
+
+Lemma vt_with_args_cast vt params srts ty:
+  (forall x, In x (type_vars ty) -> In x params) ->
+  NoDup params ->
+  length srts = length params ->
+  v_subst (vt_with_args vt params srts) ty =
+  ty_subst_s params srts ty.
+Proof.
+  intros. apply v_ty_subst_eq; auto.
+  intros. apply vt_with_args_nth; auto.
+Qed.
+
+Lemma recfun_in_funsyms {f: funsym} {l: list funpred_def}
+  (l_in: In l (mutfuns_of_context gamma))
+  (f_in: funsym_in_mutfun f l):
+  In f (funsyms_of_context gamma).
+Proof.
+  unfold funsyms_of_context. rewrite in_concat.
+  exists (funsyms_of_def (recursive_def l)).
+  split. rewrite in_map_iff. exists (recursive_def l).
+  split; auto. apply in_mutfuns_spec in l_in; auto.
+  apply in_bool_In in f_in. auto.
+Qed.
+
+(*NOTE: really could just require f in funsyms_of_context gamma*)
+Lemma funs_cast vt {f: funsym} {srts}
+  (f_in: In f (funsyms_of_context gamma)):
+  length srts = length (s_params f) ->
+  v_subst (vt_with_args vt (s_params f) srts) (f_ret f) = 
+  funsym_sigma_ret f srts.
+Proof.
+  intros.
+  unfold funsym_sigma_ret.
+  apply vt_with_args_cast; auto.
+  2: apply s_params_Nodup.
+  destruct gamma_valid as [Hwf _].
+  destruct Hwf as [Hwf [_ [Hfin _]]].
+  rewrite Forall_forall in Hfin.
+  specialize (Hfin _ f_in).
+  destruct Hwf as [Hwff _].
+  rewrite Forall_forall in Hwff.
+  specialize (Hwff _ Hfin). rewrite Forall_forall in Hwff.
+  specialize (Hwff (f_ret f) (ltac:(simpl; auto))).
+  destruct Hwff as [_ Hall].
+  rewrite Forall_forall in Hall. apply Hall.
+Qed.
+
+(*TODO: move*)
+Lemma funpred_with_reps_funs_notin {pf} {l: list funpred_def}
+  (l_in: In l (mutfuns_of_context gamma))
+  (il: list nat)
+  : length l = length il ->
+forall (f : funsym) (srts : list sort) (a : arg_list domain (sym_sigma_args f srts)),
+~
+In f
+  (map fn_sym
+     (map
+        (fun x : funsym * list vsymbol * term * nat =>
+         fundef_to_fn (fst (fst (fst x))) (snd (fst (fst x))) (snd (fst x)) (snd x))
+        (combine (fst (split_funpred_defs l))
+           (firstn (Datatypes.length (fst (split_funpred_defs l))) 
+           il)))) ->
+funs gamma_valid pd pf f srts a =
+funs gamma_valid pd (funpred_with_reps pf l l_in) f srts a.
+Proof.
+  intros. simpl.
+  unfold funpred_with_reps_funs.
+  destruct (funsym_in_mutfun_dec f l); auto.
+  destruct (Nat.eq_dec (length srts) (length (s_params f))); auto.
+  (*Here is the contradiction*)
+  exfalso.
+  destruct (get_funsym_fn l_in i H) as [f' [Hinf' Hf]]; subst.
+  apply H0. rewrite in_map_iff. exists f'. split; auto.
+Qed.
+
+Lemma funpred_with_reps_preds_notin {pf} {l: list funpred_def}
+  (l_in: In l (mutfuns_of_context gamma))
+  (il: list nat)
+  : length l = length il ->
+  forall (p : predsym) (srts : list sort) (a : arg_list domain (sym_sigma_args p srts)),
+  ~
+  In p
+    (map pn_sym
+       (map
+          (fun x : predsym * list vsymbol * formula * nat =>
+           preddef_to_pn (fst (fst (fst x))) (snd (fst (fst x))) (snd (fst x)) (snd x))
+          (combine (snd (split_funpred_defs l))
+             (skipn (Datatypes.length (fst (split_funpred_defs l))) il)))) ->
+  preds gamma_valid pd pf p srts a =
+  preds gamma_valid pd (funpred_with_reps pf l l_in) p srts a.
+Proof.
+  intros. simpl.
+  unfold funpred_with_reps_preds.
+  destruct (predsym_in_mutfun_dec p l); auto.
+  destruct (Nat.eq_dec (length srts) (length (s_params p))); auto.
+  (*Here is the contradiction*)
+  exfalso.
+  destruct (get_predsym_pn l_in i H) as [f' [Hinf' Hf]]; subst.
+  apply H0. rewrite in_map_iff. exists f'. split; auto.
+Qed.
+
+Lemma vt_with_args_in_eq (ty: vty) (vt1 vt2: val_typevar)
+  params srts:
+  length params = length srts ->
+  NoDup params ->
+  (forall x, In x (type_vars ty) -> In x params) ->
+  v_subst (vt_with_args vt1 params srts) ty =
+  v_subst (vt_with_args vt2 params srts) ty.
+Proof.
+  intros.
+  apply v_subst_ext.
+  intros.
+  apply H1 in H2.
+  destruct (In_nth _ _ EmptyString H2) as [i [Hi Hx]]; subst.
+  rewrite !vt_with_args_nth; auto.
+Qed.
+
+(*Now, we can state our spec:*)
+Theorem funs_rep_spec (pf: pi_funpred gamma_valid pd)
+  (l: list funpred_def)
+  (l_in: In l (mutfuns_of_context gamma)):
+  forall (f: funsym) (args: list vsymbol) (body: term)
+  (f_in: In (fun_def f args body) l)
+  (srts: list sort) (srts_len: length srts = length (s_params f))
+  (a: arg_list domain (sym_sigma_args f srts))
+  (vt: val_typevar) (vv: val_vars pd vt),
+  funs_rep pf f l (fun_in_mutfun f_in) l_in srts srts_len a =
+  (*We need a cast because we change [val_typevar]*)
+  dom_cast _ (funs_cast vt (recfun_in_funsyms l_in (fun_in_mutfun f_in)) srts_len) (
+  (*The function is the same as evaluating the body*)
+  term_rep gamma_valid pd all_unif 
+  (*Setting the function params to srts*)
+  (vt_with_args vt (s_params f) srts)
+  (*And recursively using [funs_rep] and [preds_rep]*)
+  (funpred_with_reps pf l l_in)
+  (*And setting the function arguments to a*)
+  (val_with_args _ _ (upd_vv_args vt vv (s_params f) srts (eq_sym srts_len)
+    (s_params_Nodup _)) args a)
+  (*Evaluating the function body*)
+  body (f_ret f) (f_body_type l_in f_in)).
+Proof.
+  intros.
+  unfold funs_rep. simpl.
+  destruct (funpred_def_valid l l_in) as [Hallval Hex].
+  destruct (Typechecker.funpred_def_term_decide sigma gamma (proj1 gamma_valid) l l_in Hex) as [t Ht].
+  unfold funpred_def_term in Ht.
+  destruct Ht as [Hnotnil [Hlenparams [m_in [Hlen [Hidx [Hfvty [Hpvty [Hfparams [Hpparams [Hfdec Hpdec]]]]]]]]]].
+  (*First step: use [funpred_with_args pf l l_in] instead of pf.
+    we are allowed to do this by [funcs_rep_aux_change_pf]*)
+  unfold funs_rep_aux. simpl.
+  rewrite funcs_rep_aux_change_pf with (pf2:=(funpred_with_reps pf l l_in)).
+  2: {
+    apply funpred_with_reps_funs_notin. auto.
+  }
+  2: { apply funpred_with_reps_preds_notin. auto. }
+
+  (*Simplify f*)
+  assert (Hf: f = fn_sym (proj1_sig (get_funsym_fn l_in (fun_in_mutfun f_in) (eq_sym Hlen)))). {
+    destruct ((get_funsym_fn l_in (fun_in_mutfun f_in) (eq_sym Hlen))); simpl.
+    apply a0.
+  }
+  assert (Hparams: snd (fst (fst t)) = s_params f). {
+    rewrite Hf. 
+    erewrite <- Hfparams. reflexivity.
+    destruct (get_funsym_fn l_in (fun_in_mutfun f_in) (eq_sym Hlen)); simpl.
+    apply a0.
+  }
+  destruct t as [[[m params] vs] il]. simpl in *.
+  generalize dependent ((get_funsym_fn l_in (fun_in_mutfun f_in) (eq_sym Hlen))).
+  intros [f' [Hinf' Hf1]] Hf2. subst. clear Hf2.
+  simpl.
+  (*Now our pf's are the same, so we use [funpred_rep_aux_eq]*)
+  (*TODO: find which vv to use*)
+  erewrite funpred_rep_aux_eq. simpl.
+  - rewrite !dom_cast_compose.
+    (*Now, need to deal with all the casting*) 
+(*So we need to know that (v_subst (vt_with_args triv_val_typevar params srts) ty =
+  v_subst (vt_with_args vt params srts) ty)*)
+assert (Hv: (v_subst (vt_with_args vt (s_params (fn_sym f')) srts) (f_ret (fn_sym f'))) =
+(v_subst (vt_with_args triv_val_typevar (s_params (fn_sym f')) srts)
+(f_ret (fn_sym f')))).
+{
+  apply vt_with_args_in_eq; auto.
+  apply s_params_Nodup.
+  intros x Hinx.
+  apply (@funpred_defs_to_sns_typevars1 l il) with(f:=f')(ty:=(f_ret (fn_sym f')));
+  auto. simpl; auto.
+}
+(*Now these are the same type*)
+match goal with
+| |- dom_cast ?d ?H1 ?t1 = dom_cast ?d ?H2 ?t2 =>
+  assert (t1 = dom_cast (dom_aux pd) Hv t2)
+end.
+2: {
+  rewrite H.
+  rewrite !dom_cast_compose.
+  apply dom_cast_eq.
+}
+(*Ok, now we need to prove this*)
+(*First, simplify cast*)
+unfold cast_arg_list. rewrite !eq_trans_refl_l.
+rewrite !scast_scast. rewrite <- !eq_sym_map_distr.
+rewrite eq_trans_sym_inv_r.
+(*Now we need to transform these, since they use
+  different [val_typevar]s. We use [vt_fv_agree_tm]*)
+assert (body = fn_body f'). {
+  admit.
+}
+assert (args = sn_args f') by admit.
+subst.
+rewrite (term_rep_irrel) with(Hty2:=f_body_type l_in f_in).
+apply vt_fv_agree_tm.
++ intros x Hinx.
+  (*TODO: require in typing that tm_type_vars body is a
+    subset of params (or s_params)*)
+  assert (In x (s_params (fn_sym f'))) by admit.
+  destruct (In_nth _ _ EmptyString H) as [i [Hi Hx]]; subst.
+  rewrite !vt_with_args_nth; auto; apply s_params_Nodup.
++ intros x Hinx Heq.
+  (*Here, we prove that the valuations for all free vars
+    are equal*)
+  (*Should have: all free vars are in args - can prove, TODO*)
+  assert (In x (sn_args f')) by admit.
+  destruct (In_nth _ _ vs_d H) as [i [ Hi Hx]]; subst.
+  assert (Hargs: s_args (fn_sym f') = map snd (sn_args f')). {
+    rewrite Forall_forall in Hallval; apply Hallval in f_in.
+    simpl in f_in. symmetry. apply f_in.
+  }
+  assert (Heq1: forall vt, nth i (sym_sigma_args (fn_sym f') srts) s_int =
+  v_subst (vt_with_args vt (s_params (fn_sym f')) srts) (snd (nth i (sn_args f') vs_d))). {
+    intros vt1.
+    unfold sym_sigma_args.  unfold ty_subst_list_s.
+    rewrite map_nth_inbound with(d2:=vty_int); [| rewrite Hargs, map_length; auto].
+    erewrite <- vt_with_args_cast with(vt:=vt1); auto.
+    - rewrite Hargs. rewrite map_nth_inbound with(d2:=vs_d); auto.
+    - intros. 
+      apply (@funpred_defs_to_sns_typevars1 l il) with(f:=f')(ty:=(nth i (s_args (fn_sym f')) vty_int));
+      auto. simpl; auto. right.
+      apply nth_In. rewrite Hargs, map_length; auto.
+    - apply s_params_Nodup.
+  }
+  rewrite val_with_args_in with (Heq:=Heq1 vt); auto.
+  (*TODO: other goals*)
+  2: {
+    rewrite Forall_forall in Hallval. apply Hallval in f_in.
+    simpl in f_in. destruct_all. apply NoDup_map_inv in H2; auto. 
+  }
+  2: {
+    unfold sym_sigma_args, ty_subst_list_s.
+    rewrite map_length, Hargs, map_length.
+    reflexivity.
+  }
+  (*Now we need to rewrite the other one*)
+  rewrite val_with_args_in with(Heq:=Heq1 triv_val_typevar); auto.
+  (*TODO: separate out*)
+  2: {
+    rewrite Forall_forall in Hallval. apply Hallval in f_in.
+    simpl in f_in. destruct_all. apply NoDup_map_inv in H2; auto. 
+  }
+  2: {
+    unfold sym_sigma_args, ty_subst_list_s.
+    rewrite map_length, Hargs, map_length.
+    reflexivity.
+  }
+  rewrite !dom_cast_compose.
+  simpl. apply dom_cast_eq.
+- (*Now we have to prove that the function values are correct*)
+  (*TODO: should be separate lemma*)
+  intros. simpl.
+  unfold funpred_with_reps_funs.
+  destruct (funsym_in_mutfun_dec (fn_sym f) l).
+  + destruct (Nat.eq_dec (Datatypes.length srts0) (Datatypes.length (s_params (fn_sym f)))).
+    * unfold funs_rep. simpl.
+      destruct (funpred_def_valid l l_in) as [Hallval' Hex'].
+      destruct (Typechecker.funpred_def_term_decide sigma gamma (proj1 gamma_valid) l l_in Hex') as [t1 Ht1].
+      unfold funpred_def_term in Ht1.
+      destruct Ht1 as [Hnotnil1 [Hlenparams1 [m_in1 [Hlen1 [Hidx1 [Hfvty1 [Hpvty1 [Hfparams1 [Hpparams1 [Hfdec1 Hpdec1]]]]]]]]]].
+      simpl.
+      assert (Hf: f = (proj1_sig (get_funsym_fn l_in i (eq_sym Hlen1)))). {
+        destruct ((get_funsym_fn l_in i (eq_sym Hlen1))); simpl.
+        (*Use uniqueness*)
+        destruct a1.
+        (*Ugh, the does follow but it is annoying*)
+        admit.
+      }
+      (*TODO: start here (then go back and prove admitted)*)
+
+      (*
+      clear f_in0.
+      assert (Hparams: snd (fst (fst t1)) = s_params f). {
+        rewrite Hf. 
+        erewrite <- Hfparams. reflexivity.
+        destruct (get_funsym_fn l_in (fun_in_mutfun f_in) (eq_sym Hlen)); simpl.
+        apply a0.
+      }
+      destruct t as [[[m params] vs] il]. simpl in *.
+      generalize dependent ((get_funsym_fn l_in (fun_in_mutfun f_in) (eq_sym Hlen))).
+      intros [f' [Hinf' Hf1]] Hf2. subst. clear Hf2.
+      simpl.
+      subst.
+      generalize dependent ((get_funsym_fn l_in i (eq_sym Hlen1))).
+      intros [f'' [Hinf'' Hf2]] Hf3. subst. clear Hf3.
+      simpl.
+      assert ()
+      Check (f_equal (fun x : funsym => funsym_sigma_ret x srts0)
+      (eq_sym (proj2 (conj Hinf'' Hf2)))).
+      Check (f_equal (fun x : funsym => funsym_sigma_ret x srts0)
+      (eq_sym (proj2 (proj2_sig (get_funsym_fn l_in i (eq_sym Hlen1)))))).
+      Check (f_equal (fun x : funsym => funsym_sigma_ret x srts0)
+      (eq_sym (proj2 (proj2_sig (get_funsym_fn l_in i (eq_sym Hlen1)))))).
+
+
+  unfold funpred_with_reps.
+   simpl.
+  unfold funs_rep_aux.
+  Unshelve.
+  [| apply s_params_Nodup|].
+  Unshelve.
+  Search val_with_args.
+
+
+  val_with_args_in:
+  forall {pd : pi_dom} (m : mut_adt) (vs : list vty),
+  Datatypes.length vs = Datatypes.length (m_params m) ->
+  forall (vt : val_typevar) (vv : val_vars pd vt) 
+	(vars : list vsymbol) (srts : list sort)
+    (a : arg_list (IndTypes.domain (dom_aux pd)) srts),
+  NoDup vars ->
+  Datatypes.length vars = Datatypes.length srts ->
+  forall i : nat,
+  i < Datatypes.length vars ->
+  forall Heq : nth i srts s_int = v_subst vt (snd (nth i vars vs_d)),
+  val_with_args vt vv vars a (nth i vars vs_d) =
+  dom_cast (dom_aux pd) Heq (hnth i a s_int (dom_int pd))
+
+
+
+
+(*Now we show that the valuation*)
+
+Search eq_trans eq_sym.
+Search f_equal eq_sym.
+rewrite !eq_trans_map_distr.
+Search eq_trans f_equal.
+
+unfold proj2.
+
+
+simpl.
+
+vt_with_args_in_eq
+
+  
+  unfold funs_rep_aux.
+  (*TODO: need to prove, rewrite with other pf first*)
+  erewrite funpred_rep_aux_eq. simpl.
+  Search funs_rep_aux.
+  simpl.*)
+Admitted.
+
+(*The pred spec is easier, we don't need a cast*)
+Theorem preds_rep_spec (pf: pi_funpred gamma_valid pd)
+  (l: list funpred_def)
+  (l_in: In l (mutfuns_of_context gamma)):
+  forall (p: predsym) (args: list vsymbol) (body: formula)
+  (p_in: In (pred_def p args body) l)
+  (srts: list sort) (srts_len: length srts = length (s_params p))
+  (a: arg_list domain (sym_sigma_args p srts))
+  (vt: val_typevar) (vv: val_vars pd vt),
+  preds_rep pf p l (pred_in_mutfun p_in) l_in srts srts_len a =
+  (*The function is the same as evaluating the body*)
+  formula_rep gamma_valid pd all_unif 
+  (*Setting the function params to srts*)
+  (vt_with_args vt (s_params p) srts)
+  (*And recursively using [funs_rep] and [preds_rep]*)
+  (funpred_with_reps pf l l_in)
+  (*And setting the function arguments to a*)
+  (val_with_args _ _ (upd_vv_args vt vv (s_params p) srts (eq_sym srts_len)
+    (s_params_Nodup _)) args a)
+  (*Evaluating the function body*)
+  body (p_body_type l_in p_in).
+Proof.
+Admitted.
+
+
+End Full.
